Progress on canon_semiring

ulib/FStar.Tactics.CanonCommSemiring.fst
@@ -15,104 +15,121 @@
 *)
 module FStar.Tactics.CanonCommSemiring
 
-/// A tactic to solve equalities on commutative semirings
+/// A tactic to solve equalities on a commutative semiring (a, +, *, 0, 1)
 ///
-/// This requires the following properties:
-/// - addition is commutative and associative, where zero is the additive identity
-/// - multiplication is commutative and associative, where one is the multiplicative identity
-/// - multiplication distributes over addition
+/// The tactic [canon_semiring] is parameterized by the base type [a] and
+/// a semiring theory [cr a]. This requires:
 ///
-/// Based on the legacy second version of Coq's ring tactic:
-///   https://github.com/coq-contribs/legacy-ring/
+/// - A commutative monoid (a, +, 0) for addition
+///   That is, + is associative, commutative and has identity element 0
+/// - A commutative monoid (a, *, 1) for multiplication
+///   That is, * is associative, commutative and has identity element 1
+/// - Multipication left-distributes over addition
+///   That is, a * (b + c) == a * b + a * c
+/// - 0 is an absorbing element of multiplication
+///   That is, 0 * a = 0
 ///
-/// In contrast to FStar.Tactics.CanonCommSemiring in master,
-/// the tactic defined here canonizes products and additions, gathers duplicate monomials, and eliminates trivial expressions.
+/// In contrast to the previous version of FStar.Tactics.CanonCommSemiring,
+/// the tactic defined here canonizes products and additions, collects
+/// coefficients in monomials, and eliminates trivial expressions.
+///
+/// This is based on the legacy (second) version of Coq's ring tactic:
+///  -  https://github.com/coq-contribs/legacy-ring/
+///
+/// See also the newest ring tactic in Coq, which is even more general
+/// and efficient:
+///  - https://coq.inria.fr/refman/addendum/ring.html
+///  - http://www.cs.ru.nl/~freek/courses/tt-2014/read/10.1.1.61.3041.pdf
 
 open FStar.List
 open FStar.Tactics
 open FStar.Reflection
-open FStar.Classical
 open FStar.Algebra.CommMonoid
 
-module CCM = FStar.Tactics.CanonCommMonoid
-
-(* Only dump when debugging is on *)
-let ddump m = if debugging () then dump m
-
+(** An attribute for marking definitions to unfold by the tactic *)
 irreducible let canon_attr = ()
 
-[@canon_attr]
-unfold let cm_op = CM?.mult
-
-(***** Commutative semirings *)
+///
+/// Commutative semiring theory
+///
 
 let distribute_left_lemma (a:Type) (cm_add:cm a) (cm_mult:cm a) =
-  let (+) = cm_op cm_add in
-  let ( * ) = cm_op cm_mult in
+  let ( + ) = cm_add.mult in
+  let ( * ) = cm_mult.mult in
   x:a -> y:a -> z:a -> Lemma (x * (y + z) == x * y + x * z)
 
 let distribute_right_lemma (a:Type) (cm_add:cm a) (cm_mult:cm a) =
-  let (+) = cm_op cm_add in
-  let ( * ) = cm_op cm_mult in
+  let ( + ) = cm_add.mult in
+  let ( * ) = cm_mult.mult in
   x:a -> y:a -> z:a -> Lemma ((x + y) * z == x * z + y * z)
+
+let mult_zero_l_lemma (a:Type) (cm_add:cm a) (cm_mult:cm a) =
+  x:a -> Lemma (cm_mult.mult cm_add.unit x == cm_add.unit)
 
 [@canon_attr]
 unopteq
 type cr (a:Type) =
   | CR :
-    cm_add:cm a ->
-    cm_mult:cm a ->
-    distribute:distribute_left_lemma a cm_add cm_mult ->
+    cm_add: cm a ->
+    cm_mult: cm a ->
+    distribute: distribute_left_lemma a cm_add cm_mult ->
+    mult_zero_l: mult_zero_l_lemma a cm_add cm_mult ->
     cr a
 
 let distribute_right (#a:Type) (r:cr a) : distribute_right_lemma a r.cm_add r.cm_mult =
   fun x y z ->
-    CM?.commutativity r.cm_mult (cm_op r.cm_add x y) z;
+    r.cm_mult.commutativity (r.cm_add.mult x y) z;
     r.distribute z x y;
-    CM?.commutativity r.cm_mult x z;
-    CM?.commutativity r.cm_mult y z
+    r.cm_mult.commutativity x z;
+    r.cm_mult.commutativity y z
 
+///
+/// Syntax of canonical ring expressions
+///
+
+(** 
+ * Marking expressions we would like to normalize fully.
+ * This does not do anything at the moment, but it would be nice
+ * to have a cheap mechanism to make this work without traversing the 
+ * whole goal.
+**)
 [@canon_attr]
-let int_cr : cr int =
-  CR int_plus_cm int_multiply_cm (fun x y z -> ())
+unfold let norm_fully (#a:Type) (x:a) = x
 
-(***** Expression syntax *)
+let index: eqtype = nat
 
-let index : eqtype = nat
-
-type varlist : Type =
+(*
+ * A list of variables represents a sorted product of one or more variables.
+ * We do not need to prove sortedness to prove correctness, so we never
+ *  make it explicit.
+ *)
+type varlist =
   | Nil_var : varlist
   | Cons_var : index -> varlist -> varlist
 
-type canonical_sum (a:Type) : Type =
+(*
+ * A canonical expression represents an ordered sum of monomials.
+ * Each monomial is either:
+ * - a varlist (a product of variables): x1 * ... * xk
+ * - a product of a scalar and a varlist: c * x1 * ... * xk
+ * - a monomial without a scalar plus a canonical expression x1 * ... * xk + s
+ *
+ * The order on monomials is the lexicographic order on varlist, with the
+ * additional convention that monomials with a scalar are less than monomials
+ * without a scalar.
+ *)
+type canonical_sum a =
   | Nil_monom : canonical_sum a
   | Cons_monom : a -> varlist -> canonical_sum a -> canonical_sum a
   | Cons_varlist : varlist -> canonical_sum a -> canonical_sum a
-
-(* Order on monoms *)
-
-(* That's the lexicographic order on varlist, extended by :
-  - A constant is less than every monom
-  - The relation between two varlist is preserved by multiplication by a
-  constant.
-  Examples :
-  3 < x < y
-  x*y < x*y*y*z
-  2*x*y < x*y*y*z
-  x*y < 54*x*y*y*z
-  4*x*y < 59*x*y*y*z
-*)
 
 [@canon_attr]
 let rec varlist_lt (x y:varlist) : bool =
   match x, y with
   | Nil_var, Cons_var _ _ -> true
-  | Cons_var i xrest, Cons_var j yrest ->
-      if i < j
-      then true
-      else i = j && varlist_lt xrest yrest
+  | Cons_var i xs, Cons_var j ys ->
+    if i < j then true else i = j && varlist_lt xs ys
   | _, _ -> false
-
 
 [@canon_attr]
 val varlist_merge: l1:varlist -> l2:varlist -> Tot varlist (decreases %[l1; l2; 0])
@@ -120,142 +137,122 @@ val varlist_merge: l1:varlist -> l2:varlist -> Tot varlist (decreases %[l1; l2; 
 [@canon_attr]
 val vm_aux: index -> t1:varlist -> l2:varlist -> Tot varlist (decreases %[t1; l2; 1])
 
-(* merges two variables lists *)
+(* Merges two lists of variables, preserving sortedness *)
 [@canon_attr]
 let rec varlist_merge l1 l2 =
   match l1, l2 with
-  | Cons_var v1 t1, Nil_var -> l1
-  | Cons_var v1 t1, Cons_var v2 t2 -> vm_aux v1 t1 l2
+  | _, Nil_var -> l1
   | Nil_var, _ -> l2
+  | Cons_var v1 t1, Cons_var v2 t2 -> vm_aux v1 t1 l2
 and vm_aux v1 t1 l2 =
   match l2 with
   | Cons_var v2 t2 ->
     if v1 < v2
     then Cons_var v1 (varlist_merge t1 l2)
     else Cons_var v2 (vm_aux v1 t1 t2)
- | _ -> Cons_var v1 t1
+  | _ -> Cons_var v1 t1
 
-
-(* returns the sum of two canonical sums  *)
+(*
+ * Merges two canonical expressions
+ *
+ * We require that [a] is eqtype for better reasons later.
+ * Here it is convenient to fix the universe of [a] in
+ * mutually recursive functions.
+ *)
 [@canon_attr]
-val canonical_sum_merge : #a:Type0 -> cr a -> s1:canonical_sum a
-  -> s2:canonical_sum a -> Tot (canonical_sum a) (decreases %[s1; s2; 0])
+val canonical_sum_merge : #a:eqtype -> cr a
+  -> s1:canonical_sum a -> s2:canonical_sum a
+  -> Tot (canonical_sum a) (decreases %[s1; s2; 0])
 
 [@canon_attr]
-val csm_aux: #a:Type0 -> r:cr a -> c1:a -> l1:varlist -> t1:canonical_sum a
-  -> s2:canonical_sum a -> Tot (canonical_sum a) (decreases %[t1; s2; 1])
-
-[@canon_attr]
-val csm_aux2: #a:Type0 -> r:cr a -> l1:varlist -> t1:canonical_sum a
+val csm_aux: #a:eqtype -> r:cr a -> c1:a -> l1:varlist -> t1:canonical_sum a
   -> s2:canonical_sum a -> Tot (canonical_sum a) (decreases %[t1; s2; 1])
 
 [@canon_attr]
 let rec canonical_sum_merge #a r s1 s2 =
-  let aplus = cm_op r.cm_add in
-  let aone = CM?.unit r.cm_mult in
+  let aplus = r.cm_add.mult in
+  let aone  = r.cm_mult.unit in
   match s1 with
-  | Cons_monom c1 l1 t1 -> csm_aux #a r c1 l1 t1 s2
-  | Cons_varlist l1 t1 -> csm_aux2 #a r l1 t1 s2
+  | Cons_monom c1 l1 t1 -> csm_aux r c1 l1 t1 s2
+  | Cons_varlist l1 t1  -> csm_aux r aone l1 t1 s2
   | Nil_monom -> s2
 
 and csm_aux #a r c1 l1 t1 s2 =
-  let aplus = cm_op r.cm_add in
-  let aone = CM?.unit r.cm_mult in
+  let aplus = r.cm_add.mult in
+  let aone  = r.cm_mult.unit in
   match s2 with
   | Cons_monom c2 l2 t2 ->
-      if l1 = l2
-      then Cons_monom (aplus c1 c2) l1 (canonical_sum_merge #a r t1 t2)
-      else
-       if varlist_lt l1 l2
-       then Cons_monom c1 l1 (canonical_sum_merge r t1 s2)
-       else Cons_monom c2 l2 (csm_aux #a r c1 l1 t1 t2)
+    if l1 = l2
+    then Cons_monom (norm_fully (aplus c1 c2)) l1 (canonical_sum_merge r t1 t2)
+    else
+      if varlist_lt l1 l2
+      then Cons_monom c1 l1 (canonical_sum_merge r t1 s2)
+      else Cons_monom c2 l2 (csm_aux #a r c1 l1 t1 t2)
   | Cons_varlist l2 t2 ->
-      if l1 = l2
-      then Cons_monom (aplus c1 aone) l1 (canonical_sum_merge r t1 t2)
-      else
-       if varlist_lt l1 l2
-       then Cons_monom c1 l1 (canonical_sum_merge r t1 s2)
-       else Cons_varlist l2 (csm_aux #a r c1 l1 t1 t2)
-  | Nil_monom -> Cons_monom c1 l1 t1
+    if l1 = l2
+    then Cons_monom (norm_fully (aplus c1 aone)) l1 (canonical_sum_merge r t1 t2)
+    else
+      if varlist_lt l1 l2
+      then Cons_monom c1 l1 (canonical_sum_merge r t1 s2)
+      else Cons_varlist l2 (csm_aux r c1 l1 t1 t2)
+  | Nil_monom ->
+    if c1 = aone
+    then Cons_varlist l1 t1
+    else Cons_monom c1 l1 t1
 
-and csm_aux2 #a r l1 t1 s2 =
-  let aplus = cm_op r.cm_add in
-  let aone = CM?.unit r.cm_mult in
-  match s2 with
-  | Cons_monom c2 l2 t2 ->
-      if l1 = l2
-      then Cons_monom (aplus aone c2) l1 (canonical_sum_merge r t1 t2)
-      else
-       if varlist_lt l1 l2
-       then Cons_varlist l1 (canonical_sum_merge r t1 s2)
-       else Cons_monom c2 l2 (csm_aux2 #a r l1 t1 t2)
-  | Cons_varlist l2 t2 ->
-      if l1 = l2
-      then Cons_monom (aplus aone aone) l1 (canonical_sum_merge r t1 t2)
-      else
-       if varlist_lt l1 l2
-       then Cons_varlist l1 (canonical_sum_merge r t1 s2)
-       else Cons_varlist l2 (csm_aux2 #a r l1 t1 t2)
-  | Nil_monom -> Cons_varlist l1 t1
-
+(* Inserts a monomial into the apropriate position in a canonical sum *)
+val monom_insert: #a:eqtype -> r:cr a
+  -> c1:a -> l1:varlist -> s2:canonical_sum a -> canonical_sum a
 
 [@canon_attr]
-let rec monom_insert (#a:Type) (r:cr a) (c1:a) (l1:varlist) (s2:canonical_sum a) :
- canonical_sum a =
-  let aplus = cm_op r.cm_add in
-  let aone = CM?.unit r.cm_add in
+let rec monom_insert #a r c1 l1 s2 =
+  let aplus = r.cm_add.mult in
+  let aone  = r.cm_mult.unit in
   match s2 with
   | Cons_monom c2 l2 t2 ->
-      if l1 = l2
-      then Cons_monom (aplus c1 c2) l1 t2
-      else
-       if varlist_lt l1 l2
-       then Cons_monom c1 l1 s2
-       else Cons_monom c2 l2 (monom_insert r c1 l1 t2)
+    if l1 = l2
+    then Cons_monom (norm_fully (aplus c1 c2)) l1 t2
+    else
+      if varlist_lt l1 l2
+      then Cons_monom c1 l1 s2
+      else Cons_monom c2 l2 (monom_insert r c1 l1 t2)
   | Cons_varlist l2 t2 ->
-      if l1 = l2
-      then Cons_monom (aplus c1 aone) l1 t2
-      else
-       if varlist_lt l1 l2
-       then Cons_monom c1 l1 s2
-       else Cons_varlist l2 (monom_insert r c1 l1 t2)
-  | Nil_monom -> Cons_monom c1 l1 Nil_monom
+    if l1 = l2
+    then Cons_monom (norm_fully (aplus c1 aone)) l1 t2
+    else
+      if varlist_lt l1 l2
+      then Cons_monom c1 l1 s2
+      else Cons_varlist l2 (monom_insert r c1 l1 t2)
+  | Nil_monom ->
+    if c1 = aone
+    then Cons_varlist l1 Nil_monom
+    else Cons_monom c1 l1 Nil_monom
+
+(* Inserts a monomial without scalar into a canonical sum *)
+val varlist_insert: #a:eqtype -> cr a -> varlist -> canonical_sum a -> canonical_sum a
 
 [@canon_attr]
-let rec varlist_insert (#a:Type) (r:cr a) (l1:varlist) (s2:canonical_sum a) :
- canonical_sum a =
-  let aplus = cm_op r.cm_add in
-  let aone = CM?.unit r.cm_add in
-  match s2 with
-  | Cons_monom c2 l2 t2 ->
-      if l1 = l2
-      then Cons_monom (aplus aone c2) l1 t2
-      else
-       if varlist_lt l1 l2
-       then Cons_varlist l1 s2
-       else Cons_monom c2 l2 (varlist_insert r l1 t2)
-  | Cons_varlist l2 t2 ->
-      if l1 = l2
-      then Cons_monom (aplus aone aone) l1 t2
-      else
-       if varlist_lt l1 l2
-       then Cons_varlist l1 s2
-       else Cons_varlist l2 (varlist_insert r l1 t2)
-  | Nil_monom -> Cons_varlist l1 Nil_monom
+let rec varlist_insert #a r l1 s2 =
+  let aone = r.cm_mult.unit in
+  monom_insert r aone l1 s2
+
+(* Multiplies a sum by a scalar c0 *)
+val canonical_sum_scalar: #a:Type -> cr a -> a -> canonical_sum a -> canonical_sum a
 
 [@canon_attr]
-let rec canonical_sum_scalar (#a:Type) (r:cr a) (c0:a) (s:canonical_sum a) :
- canonical_sum a =
-  let amult = cm_op r.cm_mult in
+let rec canonical_sum_scalar #a r c0 s =
+  let amult = r.cm_mult.mult in
   match s with
-  | Cons_monom c l t -> Cons_monom (amult c0 c) l (canonical_sum_scalar r c0 t)
+  | Cons_monom c l t -> Cons_monom (norm_fully (amult c0 c)) l (canonical_sum_scalar r c0 t)
   | Cons_varlist l t -> Cons_monom c0 l (canonical_sum_scalar r c0 t)
   | Nil_monom -> Nil_monom
 
-(* Computes l0*s  *)
+(* Multiplies a sum by a monomial without scalar *)
+val canonical_sum_scalar2: #a:eqtype -> cr a -> varlist
+  -> canonical_sum a -> canonical_sum a
+
 [@canon_attr]
-let rec canonical_sum_scalar2 (#a:Type) (r:cr a) (l0:varlist) (s:canonical_sum a) :
- canonical_sum a =
+let rec canonical_sum_scalar2 #a r l0 s =
   match s with
   | Cons_monom c l t ->
     monom_insert r c (varlist_merge l0 l) (canonical_sum_scalar2 r l0 t)
@@ -263,42 +260,54 @@ let rec canonical_sum_scalar2 (#a:Type) (r:cr a) (l0:varlist) (s:canonical_sum a
     varlist_insert r (varlist_merge l0 l) (canonical_sum_scalar2 r l0 t)
   | Nil_monom -> Nil_monom
 
-(* Computes c0*l0*s  *)
+
+(* Multiplies a sum by a monomial with scalar *)
+val canonical_sum_scalar3: #a:eqtype -> cr a -> a -> varlist
+  -> canonical_sum a -> canonical_sum a
+
 [@canon_attr]
-let rec canonical_sum_scalar3 (#a:Type) (r:cr a) (c0:a) (l0:varlist)
- (s:canonical_sum a) : canonical_sum a =
-  let amult = cm_op r.cm_mult in
+let rec canonical_sum_scalar3 #a r c0 l0 s =
+  let amult = r.cm_mult.mult in
   match s with
   | Cons_monom c l t ->
-     monom_insert r (amult c0 c) (varlist_merge l0 l)
-       (canonical_sum_scalar3 r c0 l0 t)
+    monom_insert r (norm_fully (amult c0 c)) (varlist_merge l0 l)
+                 (canonical_sum_scalar3 r c0 l0 t)
   | Cons_varlist l t ->
-     monom_insert r c0 (varlist_merge l0 l) (canonical_sum_scalar3 r c0 l0 t)
-  | Nil_monom -> Nil_monom
+    monom_insert r c0 (varlist_merge l0 l)
+                 (canonical_sum_scalar3 r c0 l0 t)
+  | Nil_monom -> s
 
-(* returns the product of two canonical sums *)
+(* Multiplies two canonical sums *)
+val canonical_sum_prod: #a:eqtype -> cr a
+  -> canonical_sum a -> canonical_sum a -> canonical_sum a
+
 [@canon_attr]
-let rec canonical_sum_prod (#a:Type) (r:cr a) (s1 s2:canonical_sum a) :
- canonical_sum a =
+let rec canonical_sum_prod #a r s1 s2 =
   match s1 with
   | Cons_monom c1 l1 t1 ->
-      canonical_sum_merge r (canonical_sum_scalar3 r c1 l1 s2)
-        (canonical_sum_prod r t1 s2)
+    canonical_sum_merge r (canonical_sum_scalar3 r c1 l1 s2)
+                          (canonical_sum_prod r t1 s2)
   | Cons_varlist l1 t1 ->
-      canonical_sum_merge r (canonical_sum_scalar2 r l1 s2)
-        (canonical_sum_prod r t1 s2)
-  | Nil_monom -> Nil_monom
+    canonical_sum_merge r (canonical_sum_scalar2 r l1 s2)
+                          (canonical_sum_prod r t1 s2)
+  | Nil_monom -> s1
 
-(* The type to represent concrete semi-ring polynomials *)
-type spolynomial (a:Type) : Type =
-  | SPvar : index -> spolynomial a
+///
+/// Syntax of concrete semiring polynomials
+///
+
+(* This is the type where we reflect expressions before normalization *)
+type spolynomial a =
+  | SPvar   : index -> spolynomial a
   | SPconst : a -> spolynomial a
-  | SPplus : spolynomial a -> spolynomial a -> spolynomial a
-  | SPmult : spolynomial a -> spolynomial a -> spolynomial a
+  | SPplus  : spolynomial a -> spolynomial a -> spolynomial a
+  | SPmult  : spolynomial a -> spolynomial a -> spolynomial a
 
+(** Canonize a reflected expression *)
+val spolynomial_normalize: #a:eqtype -> cr a -> spolynomial a -> canonical_sum a
 
 [@canon_attr]
-let rec spolynomial_normalize (#a:Type) (r:cr a) (p:spolynomial a) : canonical_sum a =
+let rec spolynomial_normalize #a r p =
   match p with
   | SPvar i -> Cons_varlist (Cons_var i Nil_var) Nil_monom
   | SPconst c -> Cons_monom c Nil_var Nil_monom
@@ -307,125 +316,203 @@ let rec spolynomial_normalize (#a:Type) (r:cr a) (p:spolynomial a) : canonical_s
   | SPmult l q ->
     canonical_sum_prod r (spolynomial_normalize r l) (spolynomial_normalize r q)
 
-(* Deletion of useless 0 and 1 in canonical sums *)
+(**
+ * Simplify a canonical sum.
+ * Removes 0 * x1 * ... * xk and turns 1 * x1 * ... * xk into x1 * ... * xk
+**)
+val canonical_sum_simplify: #a:eqtype -> cr a -> canonical_sum a -> canonical_sum a
+
 [@canon_attr]
-let rec canonical_sum_simplify (#a:eqtype) (r:cr a) (s:canonical_sum a) : canonical_sum a =
-  let azero = CM?.unit r.cm_add in
-  let aone = CM?.unit r.cm_mult in
+let rec canonical_sum_simplify #a r s =
+  let azero = r.cm_add.unit in
+  let aone  = r.cm_mult.unit in
+  let aplus = r.cm_add.mult in
   match s with
   | Cons_monom c l t ->
-      if c = azero
-      then canonical_sum_simplify r t
-      else
-       if c = aone
-       then Cons_varlist l (canonical_sum_simplify r t)
-       else Cons_monom c l (canonical_sum_simplify r t)
+    if norm_fully (c = azero) then canonical_sum_simplify r t
+    else
+      if norm_fully (c = aone)
+      then Cons_varlist l (canonical_sum_simplify r t)
+      else Cons_monom c l (canonical_sum_simplify r t)
   | Cons_varlist l t -> Cons_varlist l (canonical_sum_simplify r t)
-  | Nil_monom -> Nil_monom
+  | Nil_monom -> s
+
+(**
+ * The main canonization algorithm: turn an expression into a sum and
+ * simplify it.
+**)
+val spolynomial_simplify: #a:eqtype -> cr a -> spolynomial a -> canonical_sum a
 
 [@canon_attr]
-let spolynomial_simplify (#a:eqtype) (r:cr a) (x:spolynomial a) =
-  canonical_sum_simplify r (spolynomial_normalize r x)
+let spolynomial_simplify #a r p =
+  canonical_sum_simplify r 
+    (spolynomial_normalize r p)
 
-(* End definitions. *)
+///
+/// Interpretation of varlists, monomials and canonical sums
+///
 
-(* Section interpretation. *)
+(**
+ * The variable map:
+ * This maps polynomial variables to ring expressions. That is, any term
+ * that is not an addition or a multplication is turned into a variable
+ *
+ * The representation is inefficient. For large terms it might be worthwhile
+ * using a better data structure.
+**)
+let vmap a = list (var * a) * a
 
-(* Here a variable map is defined and the interpetation of a spolynom
-  acording to a certain variables map. Once again the choosen definition
-  is generic and could be changed *)
+(** Add a new entry in a variable map *)
+let update (#a:Type) (x:var) (xa:a) (vm:vmap a) : vmap a =
+  let l, y = vm in (x, xa) :: l, y
 
-let vmap (a:Type) = CCM.vmap a unit
+(** Quotes a list *)
+let rec quote_list (#a:Type) (ta:term) (quotea:a -> Tac term) (xs:list a) :
+    Tac term =
+  match xs with
+  | [] -> mk_app (`Nil) [(ta, Q_Implicit)]
+  | x::xs' -> mk_app (`Cons) [(ta, Q_Implicit);
+                             (quotea x, Q_Explicit);
+                             (quote_list ta quotea xs', Q_Explicit)]
 
-(* Interpretation of list of variables
- * [x1; ... ; xn ] is interpreted as (find v x1)* ... *(find v xn)
- * The unbound variables are mapped to 0. Normally this case sould
- * never occur. Since we want only to prove correctness theorems, which form
- * is : for any varmap and any spolynom ... this is a safe and pain-saving
- * choice *)
+(** Quotes a variable map *)
+let quote_vm (#a:Type) (ta: term) (quotea:a -> Tac term) (vm:vmap a) : Tac term =
+  let quote_map_entry (p:(nat * a)) : Tac term =
+    mk_app (`Mktuple2) [(`nat, Q_Implicit); (ta, Q_Implicit);
+      (pack (Tv_Const (C_Int (fst p))), Q_Explicit);
+      (quotea (snd p), Q_Explicit)] in
+  let tyentry = mk_e_app (`tuple2) [(`nat); ta] in
+  let tlist = quote_list tyentry quote_map_entry (fst vm) in
+  let tylist = mk_e_app (`list) [tyentry] in
+  mk_app (`Mktuple2) [(tylist, Q_Implicit); (ta, Q_Implicit);
+                      (tlist, Q_Explicit); (quote (snd vm), Q_Explicit)]
+
+(**
+ * A varlist is interpreted as the product of the entries in the variable map
+ *
+ * Unbound variables are mapped to the default value according to the map.
+ * This would normally never occur, but it makes it easy to prove correctness.
+ *)
 [@canon_attr]
 let interp_var (#a:Type) (vm:vmap a) (i:index) =
-  match assoc i (fst vm) with
-  | Some (x, _) -> x
-  | _ -> fst (snd vm)
+  match List.Tot.assoc i (fst vm) with
+  | Some x -> x
+  | _ -> snd vm
 
 [@canon_attr]
 private
 let rec ivl_aux (#a:Type) (r:cr a) (vm:vmap a) (x:index) (t:varlist)
   : Tot a (decreases t) =
-  let amult = cm_op r.cm_mult in
+  let amult = r.cm_mult.mult in
   match t with
   | Nil_var -> interp_var vm x
   | Cons_var x' t' -> amult (interp_var vm x) (ivl_aux r vm x' t')
 
 [@canon_attr]
 let interp_vl (#a:Type) (r:cr a) (vm:vmap a) (l:varlist) =
-  let aone = CM?.unit r.cm_mult in
+  let aone  = r.cm_mult.unit in
   match l with
   | Nil_var -> aone
   | Cons_var x t -> ivl_aux r vm x t
 
 [@canon_attr]
-private
 let rec interp_m (#a:Type) (r:cr a) (vm:vmap a) (c:a) (l:varlist) =
-  let amult = cm_op r.cm_mult in
+  let amult = r.cm_mult.mult in
   match l with
   | Nil_var -> c
   | Cons_var x t -> amult c (ivl_aux r vm x t)
 
 [@canon_attr]
-private
 let rec ics_aux (#a:Type) (r:cr a) (vm:vmap a) (x:a) (s:canonical_sum a)
   : Tot a (decreases s) =
-  let aplus = cm_op r.cm_add in
+  let aplus = r.cm_add.mult in
   match s with
   | Nil_monom -> x
   | Cons_varlist l t -> aplus x (ics_aux r vm (interp_vl r vm l) t)
   | Cons_monom c l t -> aplus x (ics_aux r vm (interp_m r vm c l) t)
 
-(* Interpretation of a canonical sum *)
+(** Interpretation of a canonical sum *)
 [@canon_attr]
 let interp_cs (#a:Type) (r:cr a) (vm:vmap a) (s:canonical_sum a) : a =
-  let azero = CM?.unit r.cm_add in
+  let azero = r.cm_add.unit in
   match s with
   | Nil_monom -> azero
   | Cons_varlist l t -> ics_aux r vm (interp_vl r vm l) t
   | Cons_monom c l t -> ics_aux r vm (interp_m r vm c l) t
 
+(** Interpretation of a polynomial *)
 [@canon_attr]
 let rec interp_sp (#a:Type) (r:cr a) (vm:vmap a) (p:spolynomial a) : a =
-  let aplus = cm_op r.cm_add in
-  let amult = cm_op r.cm_mult in
+  let aplus = r.cm_add.mult in
+  let amult = r.cm_mult.mult in
   match p with
   | SPconst c -> c
   | SPvar i -> interp_var vm i
   | SPplus p1 p2 -> aplus (interp_sp r vm p1) (interp_sp r vm p2)
   | SPmult p1 p2 -> amult (interp_sp r vm p1) (interp_sp r vm p2)
 
-(* End interpretation. *)
+///
+/// Proof of correctness
+///
 
-val ivl_aux_ok (#a:eqtype) (r:cr a) (vm:vmap a) (v:varlist) (i:index) : Lemma
-  (ivl_aux r vm i v == cm_op r.cm_mult (interp_var vm i) (interp_vl r vm v))
-let ivl_aux_ok #a r vm v i =
-  match v with
-  | Nil_var ->
-    begin
-    CM?.commutativity r.cm_mult (CM?.unit r.cm_mult) (interp_var vm i);
-    CM?.identity r.cm_mult (interp_var vm i)
-    end
-  | Cons_var x xs -> ()
+val mult_one_l (#a:Type) (r:cr a) (x:a) :
+  Lemma (r.cm_mult.mult r.cm_mult.unit x == x)
+  [SMTPat (r.cm_mult.mult r.cm_mult.unit x)]
+let mult_one_l #a r x =
+  r.cm_mult.identity x
+
+val mult_one_r (#a:Type) (r:cr a) (x:a) :
+  Lemma (r.cm_mult.mult x r.cm_mult.unit == x)
+  [SMTPat (r.cm_mult.mult x r.cm_mult.unit)]
+let mult_one_r #a r x =
+  r.cm_mult.commutativity r.cm_mult.unit x
+
+val mult_zero_l (#a:Type) (r:cr a) (x:a) :
+  Lemma (r.cm_mult.mult r.cm_add.unit x == r.cm_add.unit)
+  [SMTPat (r.cm_mult.mult r.cm_add.unit x)]
+let mult_zero_l #a r x =
+  r.mult_zero_l x
+
+val mult_zero_r (#a:Type) (r:cr a) (x:a) :
+  Lemma (r.cm_mult.mult x r.cm_add.unit == r.cm_add.unit)
+  [SMTPat (r.cm_mult.mult x r.cm_add.unit)]
+let mult_zero_r #a r x =
+  r.cm_mult.commutativity x r.cm_add.unit
+
+val add_zero_l (#a:Type) (r:cr a) (x:a) :
+  Lemma (r.cm_add.mult r.cm_add.unit x == x)
+  [SMTPat (r.cm_add.mult r.cm_add.unit x)]
+let add_zero_l #a r x =
+  r.cm_add.identity  x
+
+val add_zero_r (#a:Type) (r:cr a) (x:a) :
+  Lemma (r.cm_add.mult x r.cm_add.unit == x)
+  [SMTPat (r.cm_add.mult x r.cm_add.unit)]
+let add_zero_r #a r x =
+  r.cm_add.commutativity r.cm_add.unit x
+
+val ivl_aux_ok (#a:Type) (r:cr a) (vm:vmap a) (v:varlist) (i:index) : Lemma
+  (ivl_aux r vm i v == r.cm_mult.mult (interp_var vm i) (interp_vl r vm v))
+let ivl_aux_ok #a r vm v i = ()
+
+val vm_aux_ok (#a:eqtype) (r:cr a) (vm:vmap a) (v:index) (t l:varlist) :
+  Lemma
+  (ensures
+    interp_vl r vm (vm_aux v t l) ==
+    r.cm_mult.mult (interp_vl r vm (Cons_var v t)) (interp_vl r vm l))
+  (decreases %[t; l; 1])
 
 val varlist_merge_ok (#a:eqtype) (r:cr a) (vm:vmap a) (x y:varlist) :
-  Lemma (interp_vl r vm (varlist_merge x y) ==
-         cm_op r.cm_mult (interp_vl r vm x) (interp_vl r vm y))
+  Lemma
+  (ensures
+    interp_vl r vm (varlist_merge x y) ==
+    r.cm_mult.mult (interp_vl r vm x) (interp_vl r vm y))
+  (decreases %[x; y; 0])
+
 let rec varlist_merge_ok #a r vm x y =
-  let amult = cm_op r.cm_mult in
+  let amult = r.cm_mult.mult in
   match x, y with
-  | Cons_var v1 t1, Nil_var ->
-    begin
-    CM?.identity r.cm_mult (interp_vl r vm x);
-    CM?.commutativity r.cm_mult (CM?.unit r.cm_mult) (interp_vl r vm x)
-    end
+  | Cons_var v1 t1, Nil_var -> ()
   | Cons_var v1 t1, Cons_var v2 t2 ->
     if v1 < v2
     then
@@ -434,57 +521,72 @@ let rec varlist_merge_ok #a r vm x y =
       assert (
         interp_vl r vm (varlist_merge x y) ==
         amult (interp_var vm v1) (amult (interp_vl r vm t1) (interp_vl r vm y)));
-      CM?.associativity r.cm_mult
+      r.cm_mult.associativity
         (interp_var vm v1) (interp_vl r vm t1) (interp_vl r vm y)
       end
     else
+      vm_aux_ok r vm v1 t1 y
+  | Nil_var, _ -> ()
+and vm_aux_ok #a r vm v1 t1 l2 =
+  match l2 with
+  | Cons_var v2 t2 ->
+    if v1 < v2
+    then
       begin
-      varlist_merge_ok r vm t1 t2;
-      assert (
-        interp_vl r vm (varlist_merge x y) ==
-        amult (interp_var vm v2) (interp_vl r vm (vm_aux v1 t1 t2)));
-      ivl_aux_ok r vm t1 v1;
-      ivl_aux_ok r vm t2 v2;
-      CM?.associativity r.cm_mult
-        (interp_var vm v2) (interp_vl r vm t1) (interp_vl r vm t2);
-       admit()
+      varlist_merge_ok r vm t1 l2;
+      r.cm_mult.associativity
+        (interp_var vm v1) (interp_vl r vm t1) (interp_vl r vm l2)
       end
-  | Nil_var, _ ->
-    begin
-    CM?.identity r.cm_mult (interp_vl r vm y);
-    CM?.commutativity r.cm_mult (CM?.unit r.cm_mult) (interp_vl r vm y)
-    end
+    else
+      begin
+      vm_aux_ok r vm v1 t1 t2;
+      calc (==) {
+        interp_vl r vm (Cons_var v2 (vm_aux v1 t1 t2));
+        == { }
+        ivl_aux r vm v2 (vm_aux v1 t1 t2);
+        == { }
+        r.cm_mult.mult (interp_var vm v2) (interp_vl r vm (vm_aux v1 t1 t2));
+        == { }
+        r.cm_mult.mult (interp_var vm v2) (r.cm_mult.mult (interp_vl r vm (Cons_var v1 t1)) (interp_vl r vm t2));
+        == { r.cm_mult.commutativity
+               (interp_vl r vm (Cons_var v1 t1)) (interp_vl r vm t2) }
+        r.cm_mult.mult (interp_var vm v2)
+          (r.cm_mult.mult (interp_vl r vm t2) (interp_vl r vm (Cons_var v1 t1)) );
+        == { r.cm_mult.associativity
+              (interp_var vm v2)
+              (interp_vl r vm t2) (interp_vl r vm (Cons_var v1 t1)) }
+        r.cm_mult.mult
+         (r.cm_mult.mult (interp_var vm v2) (interp_vl r vm t2))
+         (interp_vl r vm (Cons_var v1 t1));
+        == { r.cm_mult.commutativity
+            (interp_vl r vm (Cons_var v1 t1)) (interp_vl r vm (Cons_var v2 t2)) }
+        r.cm_mult.mult (interp_vl r vm (Cons_var v1 t1)) (interp_vl r vm (Cons_var v2 t2));
+      }
+      end
+  | _ -> ()
 
-val ics_aux_ok: #a:Type -> r:cr a -> vm:vmap a -> x:a -> s:canonical_sum a ->
-  Lemma (ensures ics_aux r vm x s == cm_op r.cm_add x (interp_cs r vm s))
+val ics_aux_ok: #a:eqtype -> r:cr a -> vm:vmap a -> x:a -> s:canonical_sum a ->
+  Lemma (ensures ics_aux r vm x s == r.cm_add.mult x (interp_cs r vm s))
   (decreases s)
 let rec ics_aux_ok #a r vm x s =
   match s with
-  | Nil_monom ->
-    CM?.identity r.cm_add x;
-    CM?.commutativity r.cm_add x (CM?.unit r.cm_add)
+  | Nil_monom -> ()
   | Cons_varlist l t ->
     ics_aux_ok r vm (interp_vl r vm l) t
   | Cons_monom c l t ->
     ics_aux_ok r vm (interp_m r vm c l) t
 
-val interp_m_ok: #a:Type -> r:cr a -> vm:vmap a -> x:a -> l:varlist ->
-  Lemma (interp_m r vm x l == cm_op r.cm_mult x (interp_vl r vm l))
-let interp_m_ok #a r vm x l =
-  match l with
-  | Nil_var ->
-    CM?.identity r.cm_mult x;
-    CM?.commutativity r.cm_mult x (CM?.unit r.cm_mult)
-  | _ -> ()
-
+val interp_m_ok: #a:eqtype -> r:cr a -> vm:vmap a -> x:a -> l:varlist ->
+  Lemma (interp_m r vm x l == r.cm_mult.mult x (interp_vl r vm l))
+let interp_m_ok #a r vm x l = ()
 
 val aplus_assoc_4: #a:Type -> r:cr a -> w:a -> x:a -> y:a -> z:a -> Lemma
-  (let aplus = cm_op r.cm_add in
+  (let aplus = r.cm_add.mult in
    aplus (aplus w x) (aplus y z) == aplus (aplus w y) (aplus x z))
 let aplus_assoc_4 #a r w x y z =
-  let aplus = cm_op r.cm_add in
-  let assoc = CM?.associativity r.cm_add in
-  let comm = CM?.commutativity r.cm_add in
+  let aplus = r.cm_add.mult in
+  let assoc = r.cm_add.associativity in
+  let comm = r.cm_add.commutativity in
   calc (==) {
     aplus (aplus w x) (aplus y z);
     == { assoc w x (aplus y z) }
@@ -501,103 +603,706 @@ let aplus_assoc_4 #a r w x y z =
     aplus (aplus w y) (aplus x z);
   }
 
-val canonical_sum_merge_ok: #a:Type -> r:cr a -> vm:vmap a -> x:canonical_sum a -> y:canonical_sum a ->
-  Lemma (interp_cs r vm (canonical_sum_merge r x y) ==
-         cm_op r.cm_add (interp_cs r vm x) (interp_cs r vm y))
-let rec canonical_sum_merge_ok #a r vm x y =
-  let aplus = cm_op r.cm_add in
-  let aone = CM?.unit r.cm_mult in
-  let amult = cm_op r.cm_mult in
-  match x with
-  | Nil_monom ->
-    CM?.identity r.cm_add (interp_cs r vm y);
-    CM?.commutativity r.cm_add (interp_cs r vm y) (CM?.unit r.cm_add)
-  | Cons_monom c1 l1 t1 ->
-    begin
-    match y with
-    | Nil_monom ->
-      CM?.identity r.cm_add (interp_cs r vm x);
-      CM?.commutativity r.cm_add (interp_cs r vm x) (CM?.unit r.cm_add)
+val canonical_sum_merge_ok: #a:eqtype -> r:cr a -> vm:vmap a
+  -> s1:canonical_sum a -> s2:canonical_sum a ->
+  Lemma
+  (ensures
+    interp_cs r vm (canonical_sum_merge r s1 s2) ==
+    r.cm_add.mult (interp_cs r vm s1) (interp_cs r vm s2))
+  (decreases %[s1; s2; 0])
 
-    | Cons_monom c2 l2 t2 ->
-      if l1 = l2 then
-        begin
-        calc (==) {
-          interp_cs r vm (canonical_sum_merge r x y);
-          == { }
-          ics_aux r vm (interp_m r vm (aplus c1 c2) l1)
-                       (canonical_sum_merge r t1 t2);
-          == { ics_aux_ok r vm (interp_m r vm (aplus c1 c2) l1)
-                               (canonical_sum_merge r t1 t2) }
-          aplus (interp_m r vm (aplus c1 c2) l1)
-                (interp_cs r vm (canonical_sum_merge r t1 t2));
-          == { interp_m_ok r vm (aplus c1 c2) l1 }
-          aplus (amult (aplus c1 c2) (interp_vl r vm l1))
-                (interp_cs r vm (canonical_sum_merge r t1 t2));
-          == { canonical_sum_merge_ok r vm t1 t2 }
-          aplus (amult (aplus c1 c2) (interp_vl r vm l1))
-                (aplus (interp_cs r vm t1) (interp_cs r vm t2));
-          == { distribute_right r c1 c2 (interp_vl r vm l1) }
-          aplus (aplus (amult c1 (interp_vl r vm l1))
-                       (amult c2 (interp_vl r vm l2)))
-                (aplus (interp_cs r vm t1)
-                       (interp_cs r vm t2));
-          == { aplus_assoc_4 r
-                 (amult c1 (interp_vl r vm l1))
-                 (amult c2 (interp_vl r vm l2))
-                 (interp_cs r vm t1)
-                 (interp_cs r vm t2) }
-          aplus (aplus (amult c1 (interp_vl r vm l1)) (interp_cs r vm t1))
-                (aplus (amult c2 (interp_vl r vm l2)) (interp_cs r vm t2));
-          == { ics_aux_ok r vm (amult c1 (interp_vl r vm l1)) t1;
-               interp_m_ok r vm c1 l1 }
-          aplus (interp_cs r vm x)
-                (aplus (amult c2 (interp_vl r vm l2)) (interp_cs r vm t2));
-          == { ics_aux_ok r vm (amult c2 (interp_vl r vm l2)) t2;
-               interp_m_ok r vm c2 l2 }
-          aplus (interp_cs r vm x) (interp_cs r vm y);
-        }
-        end
-      else if varlist_lt l1 l2 then
-        begin
-        calc (==) {
-          interp_cs r vm (canonical_sum_merge r x y);
-          == { }
-          ics_aux r vm (interp_m r vm c1 l1)
-                       (canonical_sum_merge r t1 y);
-          == { ics_aux_ok r vm (interp_m r vm c1 l1)
-                               (canonical_sum_merge r t1 y) }
-          aplus (interp_m r vm c1 l1)
-                (interp_cs r vm (canonical_sum_merge r t1 y));
-          == { interp_m_ok r vm c1 l1 }
-          aplus (amult c1 (interp_vl r vm l1))
-                (interp_cs r vm (canonical_sum_merge r t1 y));
-          == { canonical_sum_merge_ok r vm t1 y }
-          aplus (amult c1 (interp_vl r vm l1))
-                (aplus (interp_cs r vm t1) (interp_cs r vm y));
-          == { admit() }
-          aplus (aplus (amult c1 (interp_vl r vm l1))
-                       (interp_cs r vm t1))
-                (interp_cs r vm y);
-          == { ics_aux_ok r vm (amult c1 (interp_vl r vm l1)) t1;
-               interp_m_ok r vm c1 l1 }
-          aplus (interp_cs r vm x) (interp_cs r vm y);
-        }
-       end
-      else admit()
-    | _ -> admit()
+val csm_aux_ok: #a:eqtype -> r:cr a -> vm:vmap a
+  -> c1:a -> l1:varlist -> t1:canonical_sum a -> s2:canonical_sum a ->
+  Lemma
+  (ensures
+    interp_cs r vm (csm_aux r c1 l1 t1 s2) ==
+    r.cm_add.mult (interp_cs r vm (Cons_monom c1 l1 t1)) (interp_cs r vm s2))
+  (decreases %[t1; s2; 1])
+
+let rec canonical_sum_merge_ok #a r vm s1 s2 =
+  let aone  = r.cm_mult.unit in
+  let aplus = r.cm_add.mult in
+  let amult = r.cm_mult.mult in
+  match s1 with
+  | Cons_monom c1 l1 t1 -> csm_aux_ok #a r vm c1 l1 t1 s2
+  | Cons_varlist l1 t1  ->
+    calc (==) {
+      interp_cs r vm (canonical_sum_merge r s1 s2);
+      == { }
+      interp_cs r vm (csm_aux r aone l1 t1 s2);
+      == { csm_aux_ok #a r vm aone l1 t1 s2 }
+      aplus (interp_cs r vm (Cons_monom aone l1 t1))
+            (interp_cs r vm s2);
+      == { ics_aux_ok r vm (interp_vl r vm l1) t1 }
+      aplus (interp_cs r vm (Cons_varlist l1 t1))
+            (interp_cs r vm s2);
+    }
+  | Nil_monom -> ()
+and csm_aux_ok #a r vm c1 l1 t1 s2 =
+  let aplus = r.cm_add.mult in
+  let aone  = r.cm_mult.unit in
+  let amult = r.cm_mult.mult in
+  match s2 with
+  | Nil_monom -> ()
+  | Cons_monom c2 l2 t2 ->
+    let s1 = Cons_monom c1 l1 t1 in
+    if l1 = l2 then
+    begin
+    calc (==) {
+      interp_cs r vm (csm_aux r c1 l1 t1 s2);
+      == { }
+      ics_aux r vm (interp_m r vm (aplus c1 c2) l1)
+                   (canonical_sum_merge r t1 t2);
+      == { ics_aux_ok r vm (interp_m r vm (aplus c1 c2) l1)
+                           (canonical_sum_merge r t1 t2) }
+      aplus (interp_m r vm (aplus c1 c2) l1)
+            (interp_cs r vm (canonical_sum_merge r t1 t2));
+      == { interp_m_ok r vm (aplus c1 c2) l1 }
+      aplus (amult (aplus c1 c2) (interp_vl r vm l1))
+            (interp_cs r vm (canonical_sum_merge r t1 t2));
+      == { canonical_sum_merge_ok r vm t1 t2 }
+      aplus (amult (aplus c1 c2) (interp_vl r vm l1))
+            (aplus (interp_cs r vm t1) (interp_cs r vm t2));
+      == { distribute_right r c1 c2 (interp_vl r vm l1) }
+      aplus (aplus (amult c1 (interp_vl r vm l1))
+                   (amult c2 (interp_vl r vm l2)))
+            (aplus (interp_cs r vm t1)
+                   (interp_cs r vm t2));
+      == { aplus_assoc_4 r
+             (amult c1 (interp_vl r vm l1))
+             (amult c2 (interp_vl r vm l2))
+             (interp_cs r vm t1)
+             (interp_cs r vm t2) }
+      aplus (aplus (amult c1 (interp_vl r vm l1)) (interp_cs r vm t1))
+            (aplus (amult c2 (interp_vl r vm l2)) (interp_cs r vm t2));
+      == { ics_aux_ok r vm (amult c1 (interp_vl r vm l1)) t1;
+           interp_m_ok r vm c1 l1 }
+      aplus (interp_cs r vm s1)
+            (aplus (amult c2 (interp_vl r vm l2)) (interp_cs r vm t2));
+      == { ics_aux_ok r vm (amult c2 (interp_vl r vm l2)) t2;
+           interp_m_ok r vm c2 l2 }
+      aplus (interp_cs r vm s1) (interp_cs r vm s2);
+    }
     end
-  | _ -> admit()
+    else if varlist_lt l1 l2 then
+    begin
+    calc (==) {
+      interp_cs r vm (canonical_sum_merge r s1 s2);
+      == { }
+      ics_aux r vm (interp_m r vm c1 l1)
+                   (canonical_sum_merge r t1 s2);
+      == { ics_aux_ok r vm (interp_m r vm c1 l1)
+                           (canonical_sum_merge r t1 s2) }
+      aplus (interp_m r vm c1 l1)
+            (interp_cs r vm (canonical_sum_merge r t1 s2));
+      == { interp_m_ok r vm c1 l1 }
+      aplus (amult c1 (interp_vl r vm l1))
+            (interp_cs r vm (canonical_sum_merge r t1 s2));
+      == { canonical_sum_merge_ok r vm t1 s2 }
+      aplus (amult c1 (interp_vl r vm l1))
+            (aplus (interp_cs r vm t1) (interp_cs r vm s2));
+      == { r.cm_add.associativity
+             (amult c1 (interp_vl r vm l1))
+             (interp_cs r vm t1)
+             (interp_cs r vm s2)
+         }
+      aplus (aplus (amult c1 (interp_vl r vm l1))
+                   (interp_cs r vm t1))
+            (interp_cs r vm s2);
+      == { ics_aux_ok r vm (amult c1 (interp_vl r vm l1)) t1;
+           interp_m_ok r vm c1 l1 }
+      aplus (interp_cs r vm s1) (interp_cs r vm s2);
+    }
+    end
+    else
+    begin
+    calc (==) {
+      interp_cs r vm (csm_aux r c1 l1 t1 s2);
+      == { }
+      ics_aux r vm (interp_m r vm c2 l2)
+                   (csm_aux r c1 l1 t1 t2);
+      == { ics_aux_ok r vm (interp_m r vm c2 l2)
+                           (csm_aux r c1 l1 t1 t2) }
+      aplus (interp_m r vm c2 l2)
+            (interp_cs r vm (csm_aux r c1 l1 t1 t2));
+      == { interp_m_ok r vm c2 l2 }
+      aplus (amult c2 (interp_vl r vm l2))
+            (interp_cs r vm (csm_aux r c1 l1 t1 t2));
+      == { csm_aux_ok r vm c1 l1 t1 t2 }
+      aplus (amult c2 (interp_vl r vm l2))
+            (aplus (interp_cs r vm s1) (interp_cs r vm t2));
+      == { r.cm_add.commutativity (interp_cs r vm s1) (interp_cs r vm t2) }
+      aplus (amult c2 (interp_vl r vm l2))
+            (aplus (interp_cs r vm t2) (interp_cs r vm s1));
+      == { r.cm_add.associativity
+             (amult c2 (interp_vl r vm l2))
+             (interp_cs r vm t2)
+             (interp_cs r vm s1)
+         }
+      aplus (aplus (amult c2 (interp_vl r vm l2))
+                   (interp_cs r vm t2))
+            (interp_cs r vm s1);
+      == { ics_aux_ok r vm (amult c1 (interp_vl r vm l1)) t1;
+           interp_m_ok r vm c1 l1 }
+      aplus (interp_cs r vm s2) (interp_cs r vm s1);
+      == { r.cm_add.commutativity (interp_cs r vm s1) (interp_cs r vm s2) }
+      aplus (interp_cs r vm s1) (interp_cs r vm s2);
+    }
+    end
+  | Cons_varlist l2 t2 -> // Same as Cons_monom with c2 = aone
+    let c2 = aone in
+    let s1 = Cons_monom c1 l1 t1 in
+    if l1 = l2 then
+    begin
+    calc (==) {
+      interp_cs r vm (csm_aux r c1 l1 t1 s2);
+      == { }
+      ics_aux r vm (interp_m r vm (aplus c1 c2) l1)
+                   (canonical_sum_merge r t1 t2);
+      == { ics_aux_ok r vm (interp_m r vm (aplus c1 c2) l1)
+                           (canonical_sum_merge r t1 t2) }
+      aplus (interp_m r vm (aplus c1 c2) l1)
+            (interp_cs r vm (canonical_sum_merge r t1 t2));
+      == { interp_m_ok r vm (aplus c1 c2) l1 }
+      aplus (amult (aplus c1 c2) (interp_vl r vm l1))
+            (interp_cs r vm (canonical_sum_merge r t1 t2));
+      == { canonical_sum_merge_ok r vm t1 t2 }
+      aplus (amult (aplus c1 c2) (interp_vl r vm l1))
+            (aplus (interp_cs r vm t1) (interp_cs r vm t2));
+      == { distribute_right r c1 c2 (interp_vl r vm l1) }
+      aplus (aplus (amult c1 (interp_vl r vm l1))
+                   (amult c2 (interp_vl r vm l2)))
+            (aplus (interp_cs r vm t1)
+                   (interp_cs r vm t2));
+      == { aplus_assoc_4 r
+             (amult c1 (interp_vl r vm l1))
+             (amult c2 (interp_vl r vm l2))
+             (interp_cs r vm t1)
+             (interp_cs r vm t2) }
+      aplus (aplus (amult c1 (interp_vl r vm l1)) (interp_cs r vm t1))
+            (aplus (amult c2 (interp_vl r vm l2)) (interp_cs r vm t2));
+      == { ics_aux_ok r vm (amult c1 (interp_vl r vm l1)) t1;
+           interp_m_ok r vm c1 l1 }
+      aplus (interp_cs r vm s1)
+            (aplus (amult c2 (interp_vl r vm l2)) (interp_cs r vm t2));
+      == { ics_aux_ok r vm (amult c2 (interp_vl r vm l2)) t2;
+           interp_m_ok r vm c2 l2 }
+      aplus (interp_cs r vm s1) (interp_cs r vm s2);
+    }
+    end
+    else if varlist_lt l1 l2 then
+    begin
+    calc (==) {
+      interp_cs r vm (canonical_sum_merge r s1 s2);
+      == { }
+      ics_aux r vm (interp_m r vm c1 l1)
+                   (canonical_sum_merge r t1 s2);
+      == { ics_aux_ok r vm (interp_m r vm c1 l1)
+                           (canonical_sum_merge r t1 s2) }
+      aplus (interp_m r vm c1 l1)
+            (interp_cs r vm (canonical_sum_merge r t1 s2));
+      == { interp_m_ok r vm c1 l1 }
+      aplus (amult c1 (interp_vl r vm l1))
+            (interp_cs r vm (canonical_sum_merge r t1 s2));
+      == { canonical_sum_merge_ok r vm t1 s2 }
+      aplus (amult c1 (interp_vl r vm l1))
+            (aplus (interp_cs r vm t1) (interp_cs r vm s2));
+      == { r.cm_add.associativity
+             (amult c1 (interp_vl r vm l1))
+             (interp_cs r vm t1)
+             (interp_cs r vm s2)
+         }
+      aplus (aplus (amult c1 (interp_vl r vm l1))
+                   (interp_cs r vm t1))
+            (interp_cs r vm s2);
+      == { ics_aux_ok r vm (amult c1 (interp_vl r vm l1)) t1;
+           interp_m_ok r vm c1 l1 }
+      aplus (interp_cs r vm s1) (interp_cs r vm s2);
+    }
+    end
+    else
+    begin
+    calc (==) {
+      interp_cs r vm (csm_aux r c1 l1 t1 s2);
+      == { }
+      ics_aux r vm (interp_m r vm c2 l2)
+                   (csm_aux r c1 l1 t1 t2);
+      == { ics_aux_ok r vm (interp_m r vm c2 l2)
+                           (csm_aux r c1 l1 t1 t2) }
+      aplus (interp_m r vm c2 l2)
+            (interp_cs r vm (csm_aux r c1 l1 t1 t2));
+      == { interp_m_ok r vm c2 l2 }
+      aplus (amult c2 (interp_vl r vm l2))
+            (interp_cs r vm (csm_aux r c1 l1 t1 t2));
+      == { csm_aux_ok r vm c1 l1 t1 t2 }
+      aplus (amult c2 (interp_vl r vm l2))
+            (aplus (interp_cs r vm s1) (interp_cs r vm t2));
+      == { r.cm_add.commutativity (interp_cs r vm s1) (interp_cs r vm t2) }
+      aplus (amult c2 (interp_vl r vm l2))
+            (aplus (interp_cs r vm t2) (interp_cs r vm s1));
+      == { r.cm_add.associativity
+             (amult c2 (interp_vl r vm l2))
+             (interp_cs r vm t2)
+             (interp_cs r vm s1)
+         }
+      aplus (aplus (amult c2 (interp_vl r vm l2))
+                   (interp_cs r vm t2))
+            (interp_cs r vm s1);
+      == { ics_aux_ok r vm (amult c1 (interp_vl r vm l1)) t1;
+           interp_m_ok r vm c1 l1 }
+      aplus (interp_cs r vm s2) (interp_cs r vm s1);
+      == { r.cm_add.commutativity (interp_cs r vm s1) (interp_cs r vm s2) }
+      aplus (interp_cs r vm s1) (interp_cs r vm s2);
+    }
+    end
+
+val monom_insert_ok: #a:eqtype -> r:cr a -> vm:vmap a
+  -> c1:a -> l1:varlist -> s2:canonical_sum a ->
+  Lemma
+  (interp_cs r vm (monom_insert r c1 l1 s2) ==
+   r.cm_add.mult (r.cm_mult.mult c1 (interp_vl r vm l1)) (interp_cs r vm s2))
+let rec monom_insert_ok #a r vm c1 l1 s2 =
+  let aplus = r.cm_add.mult in
+  let amult = r.cm_mult.mult in
+  let aone  = r.cm_mult.unit in
+  match s2 with
+  | Cons_monom c2 l2 t2 ->
+    if l1 = l2
+    then
+      calc (==) {
+        interp_cs r vm (monom_insert r c1 l1 s2);
+        == { }
+        interp_cs r vm (Cons_monom (aplus c1 c2) l1 t2);
+        == { }
+        ics_aux r vm (interp_m r vm (aplus c1 c2) l1) t2;
+        == { ics_aux_ok r vm (interp_m r vm (aplus c1 c2) l1) t2 }
+        aplus (interp_m r vm (aplus c1 c2) l1) (interp_cs r vm t2);
+        == { interp_m_ok r vm (aplus c1 c2) l1 }
+        aplus (amult (aplus c1 c2) (interp_vl r vm l2)) (interp_cs r vm t2);
+        == { distribute_right r c1 c2 (interp_vl r vm l2) }
+        aplus (aplus (amult c1 (interp_vl r vm l1))
+                     (amult c2 (interp_vl r vm l2)))
+              (interp_cs r vm t2);
+        == { r.cm_add.associativity
+               (amult c1 (interp_vl r vm l1))
+               (amult c2 (interp_vl r vm l2))
+               (interp_cs r vm t2) }
+        aplus (amult c1 (interp_vl r vm l1))
+              (aplus (amult c2 (interp_vl r vm l2))
+                     (interp_cs r vm t2));
+        == { ics_aux_ok r vm (interp_m r vm c2 l2) t2 }
+        aplus (amult c1 (interp_vl r vm l1)) (interp_cs r vm s2);
+      }
+    else
+     if varlist_lt l1 l2 then ()
+     else
+       calc (==) {
+        interp_cs r vm (monom_insert r c1 l1 s2);
+        == { }
+        interp_cs r vm (Cons_monom c2 l2 (monom_insert r c1 l1 t2));
+        == { }
+        aplus (amult c2 (interp_vl r vm l2))
+              (interp_cs r vm (monom_insert r c1 l1 t2));
+        == { monom_insert_ok r vm c1 l1 t2 }
+        aplus (amult c2 (interp_vl r vm l2))
+              (aplus (amult c1 (interp_vl r vm l1))
+                     (interp_cs r vm t2));
+        == { r.cm_add.commutativity
+               (amult c1 (interp_vl r vm l1))
+               (interp_cs r vm t2) }
+        aplus (amult c2 (interp_vl r vm l2))
+              (aplus (interp_cs r vm t2)
+                     (amult c1 (interp_vl r vm l1)));
+        == { r.cm_add.associativity
+              (amult c2 (interp_vl r vm l2))
+              (interp_cs r vm t2)
+              (amult c1 (interp_vl r vm l1)) }
+        aplus (aplus (amult c2 (interp_vl r vm l2))
+                     (interp_cs r vm t2))
+              (amult c1 (interp_vl r vm l1));
+        == { ics_aux_ok r vm (interp_m r vm c2 l2) t2 }
+        aplus (interp_cs r vm s2) (amult c1 (interp_vl r vm l1));
+        == { r.cm_add.commutativity
+              (interp_cs r vm s2)
+              (amult c1 (interp_vl r vm l1)) }
+        aplus (amult c1 (interp_vl r vm l1)) (interp_cs r vm s2);
+       }
+  | Cons_varlist l2 t2 -> // Same as Cons_monom with c2 = aone
+    let c2 = aone in
+    if l1 = l2
+    then
+      calc (==) {
+        interp_cs r vm (monom_insert r c1 l1 s2);
+        == { }
+        interp_cs r vm (Cons_monom (aplus c1 c2) l1 t2);
+        == { }
+        ics_aux r vm (interp_m r vm (aplus c1 c2) l1) t2;
+        == { ics_aux_ok r vm (interp_m r vm (aplus c1 c2) l1) t2 }
+        aplus (interp_m r vm (aplus c1 c2) l1) (interp_cs r vm t2);
+        == { interp_m_ok r vm (aplus c1 c2) l1 }
+        aplus (amult (aplus c1 c2) (interp_vl r vm l2)) (interp_cs r vm t2);
+        == { distribute_right r c1 c2 (interp_vl r vm l2) }
+        aplus (aplus (amult c1 (interp_vl r vm l1))
+                     (amult c2 (interp_vl r vm l2)))
+              (interp_cs r vm t2);
+        == { r.cm_add.associativity
+               (amult c1 (interp_vl r vm l1))
+               (amult c2 (interp_vl r vm l2))
+               (interp_cs r vm t2) }
+        aplus (amult c1 (interp_vl r vm l1))
+              (aplus (amult c2 (interp_vl r vm l2))
+                     (interp_cs r vm t2));
+        == { ics_aux_ok r vm (interp_m r vm c2 l2) t2 }
+        aplus (amult c1 (interp_vl r vm l1)) (interp_cs r vm s2);
+      }
+    else
+     if varlist_lt l1 l2 then ()
+     else
+       calc (==) {
+        interp_cs r vm (monom_insert r c1 l1 s2);
+        == { }
+        interp_cs r vm (Cons_monom c2 l2 (monom_insert r c1 l1 t2));
+        == { }
+        aplus (amult c2 (interp_vl r vm l2))
+              (interp_cs r vm (monom_insert r c1 l1 t2));
+        == { monom_insert_ok r vm c1 l1 t2 }
+        aplus (amult c2 (interp_vl r vm l2))
+              (aplus (amult c1 (interp_vl r vm l1))
+                     (interp_cs r vm t2));
+        == { r.cm_add.commutativity
+               (amult c1 (interp_vl r vm l1))
+               (interp_cs r vm t2) }
+        aplus (amult c2 (interp_vl r vm l2))
+              (aplus (interp_cs r vm t2)
+                     (amult c1 (interp_vl r vm l1)));
+        == { r.cm_add.associativity
+              (amult c2 (interp_vl r vm l2))
+              (interp_cs r vm t2)
+              (amult c1 (interp_vl r vm l1)) }
+        aplus (aplus (amult c2 (interp_vl r vm l2))
+                     (interp_cs r vm t2))
+              (amult c1 (interp_vl r vm l1));
+        == { ics_aux_ok r vm (interp_m r vm c2 l2) t2 }
+        aplus (interp_cs r vm s2) (amult c1 (interp_vl r vm l1));
+        == { r.cm_add.commutativity
+              (interp_cs r vm s2)
+              (amult c1 (interp_vl r vm l1)) }
+        aplus (amult c1 (interp_vl r vm l1)) (interp_cs r vm s2);
+       }
+  | Nil_monom -> ()
+
+val varlist_insert_ok: #a:eqtype -> r:cr a -> vm:vmap a
+  -> l1:varlist -> s2:canonical_sum a ->
+  Lemma (interp_cs r vm (varlist_insert r l1 s2) ==
+         r.cm_add.mult (interp_vl r vm l1) (interp_cs r vm s2))
+let varlist_insert_ok #a r vm l1 s2 =
+  let aone = r.cm_mult.unit in
+  monom_insert_ok r vm aone l1 s2
+
+val canonical_sum_scalar_ok: #a:eqtype -> r:cr a -> vm:vmap a
+  -> c0:a -> s:canonical_sum a ->
+  Lemma (
+    interp_cs r vm (canonical_sum_scalar r c0 s) ==
+    r.cm_mult.mult c0 (interp_cs r vm s))
+let rec canonical_sum_scalar_ok #a r vm c0 s =
+  let aone  = r.cm_mult.unit in
+  let aplus = r.cm_add.mult in
+  let amult = r.cm_mult.mult in
+  match s with
+  | Cons_monom c l t ->
+    calc (==) {
+      interp_cs r vm (canonical_sum_scalar r c0 s);
+      == { }
+      interp_cs r vm (Cons_monom (amult c0 c) l (canonical_sum_scalar r c0 t));
+      == { }
+      aplus (amult (amult c0 c) (interp_vl r vm l))
+            (interp_cs r vm (canonical_sum_scalar r c0 t));
+      == { r.cm_mult.associativity c0 c (interp_vl r vm l) }
+      aplus (amult c0 (amult c (interp_vl r vm l)))
+            (interp_cs r vm (canonical_sum_scalar r c0 t));
+      == { canonical_sum_scalar_ok r vm c0 t }
+      aplus (amult c0 (amult c (interp_vl r vm l)))
+            (amult c0 (interp_cs r vm t));
+      == { r.distribute c0 (amult c (interp_vl r vm l))
+                              (interp_cs r vm t) }
+      amult c0 (aplus (amult c (interp_vl r vm l)) (interp_cs r vm t));
+      == { }
+      amult c0 (interp_cs r vm s);
+    }
+  | Cons_varlist l t -> // Same as Cons_monom c l t with c = r.cm_mult.unit
+    let c = aone in
+        calc (==) {
+      interp_cs r vm (canonical_sum_scalar r c0 s);
+      == { }
+      interp_cs r vm (Cons_monom (amult c0 c) l (canonical_sum_scalar r c0 t));
+      == { }
+      aplus (amult (amult c0 c) (interp_vl r vm l))
+            (interp_cs r vm (canonical_sum_scalar r c0 t));
+      == { r.cm_mult.associativity c0 c (interp_vl r vm l) }
+      aplus (amult c0 (amult c (interp_vl r vm l)))
+            (interp_cs r vm (canonical_sum_scalar r c0 t));
+      == { canonical_sum_scalar_ok r vm c0 t }
+      aplus (amult c0 (amult c (interp_vl r vm l)))
+            (amult c0 (interp_cs r vm t));
+      == { r.distribute c0 (amult c (interp_vl r vm l))
+                              (interp_cs r vm t) }
+      amult c0 (aplus (amult c (interp_vl r vm l)) (interp_cs r vm t));
+      == { }
+      amult c0 (interp_cs r vm s);
+    }
+  | Nil_monom -> ()
+
+val canonical_sum_scalar2_ok: #a:eqtype -> r:cr a -> vm:vmap a
+  -> l0:varlist -> s:canonical_sum a ->
+  Lemma (
+    interp_cs r vm (canonical_sum_scalar2 r l0 s) ==
+    r.cm_mult.mult (interp_vl r vm l0) (interp_cs r vm s))
+let rec canonical_sum_scalar2_ok #a r vm l0 s =
+  let aone  = r.cm_mult.unit in
+  let aplus = r.cm_add.mult in
+  let amult = r.cm_mult.mult in
+  match s with
+  | Cons_monom c l t ->
+    calc (==) {
+      interp_cs r vm (canonical_sum_scalar2 r l0 s);
+      == { }
+      interp_cs r vm
+        (monom_insert r c (varlist_merge l0 l) (canonical_sum_scalar2 r l0 t));
+      == { monom_insert_ok r vm c (varlist_merge l0 l) (canonical_sum_scalar2 r l0 t) }
+      aplus (amult c (interp_vl r vm (varlist_merge l0 l)))
+            (interp_cs r vm (canonical_sum_scalar2 r l0 t));
+      == { varlist_merge_ok r vm l0 l }
+      aplus (amult c (amult (interp_vl r vm l0) (interp_vl r vm l)))
+            (interp_cs r vm (canonical_sum_scalar2 r l0 t));
+      == { canonical_sum_scalar2_ok r vm l0 t }
+      aplus (amult c (amult (interp_vl r vm l0) (interp_vl r vm l)))
+            (amult (interp_vl r vm l0) (interp_cs r vm t));
+      == { r.cm_mult.associativity c (interp_vl r vm l0)
+             (interp_vl r vm l) }
+      aplus (amult (amult c (interp_vl r vm l0)) (interp_vl r vm l))
+            (amult (interp_vl r vm l0) (interp_cs r vm t));
+      == { r.cm_mult.commutativity (interp_vl r vm l0) c }
+      aplus (amult (amult (interp_vl r vm l0) c) (interp_vl r vm l))
+            (amult (interp_vl r vm l0) (interp_cs r vm t));
+      == { r.cm_mult.associativity (interp_vl r vm l0) c (interp_vl r vm l) }
+      aplus (amult (interp_vl r vm l0) (amult c (interp_vl r vm l)))
+            (amult (interp_vl r vm l0) (interp_cs r vm t));
+      == { r.distribute (interp_vl r vm l0)
+             (amult c (interp_vl r vm l)) (interp_cs r vm t) }
+      amult (interp_vl r vm l0)
+            (aplus (amult c (interp_vl r vm l)) (interp_cs r vm t));
+      == {  }
+      amult (interp_vl r vm l0) (interp_cs r vm s);
+    }
+  | Cons_varlist l t -> // Same as Cons_monom c l t with c = aone
+    let c = aone in
+    calc (==) {
+      interp_cs r vm (canonical_sum_scalar2 r l0 s);
+      == { }
+      interp_cs r vm
+        (monom_insert r c (varlist_merge l0 l) (canonical_sum_scalar2 r l0 t));
+      == { monom_insert_ok r vm c (varlist_merge l0 l) (canonical_sum_scalar2 r l0 t) }
+      aplus (amult c (interp_vl r vm (varlist_merge l0 l)))
+            (interp_cs r vm (canonical_sum_scalar2 r l0 t));
+      == { varlist_merge_ok r vm l0 l }
+      aplus (amult c (amult (interp_vl r vm l0) (interp_vl r vm l)))
+            (interp_cs r vm (canonical_sum_scalar2 r l0 t));
+      == { canonical_sum_scalar2_ok r vm l0 t }
+      aplus (amult c (amult (interp_vl r vm l0) (interp_vl r vm l)))
+            (amult (interp_vl r vm l0) (interp_cs r vm t));
+      == { r.cm_mult.associativity c (interp_vl r vm l0)
+             (interp_vl r vm l) }
+      aplus (amult (amult c (interp_vl r vm l0)) (interp_vl r vm l))
+            (amult (interp_vl r vm l0) (interp_cs r vm t));
+      == { r.cm_mult.commutativity (interp_vl r vm l0) c }
+      aplus (amult (amult (interp_vl r vm l0) c) (interp_vl r vm l))
+            (amult (interp_vl r vm l0) (interp_cs r vm t));
+      == { r.cm_mult.associativity (interp_vl r vm l0) c (interp_vl r vm l) }
+      aplus (amult (interp_vl r vm l0) (amult c (interp_vl r vm l)))
+            (amult (interp_vl r vm l0) (interp_cs r vm t));
+      == { r.distribute (interp_vl r vm l0)
+             (amult c (interp_vl r vm l)) (interp_cs r vm t) }
+      amult (interp_vl r vm l0)
+            (aplus (amult c (interp_vl r vm l)) (interp_cs r vm t));
+      == {  }
+      amult (interp_vl r vm l0) (interp_cs r vm s);
+    }
+  | Nil_monom -> ()
+
+val canonical_sum_scalar3_ok: #a:eqtype -> r:cr a -> vm:vmap a
+  -> c0:a -> l0:varlist -> s:canonical_sum a ->
+  Lemma (
+    interp_cs r vm (canonical_sum_scalar3 r c0 l0 s) ==
+    r.cm_mult.mult (r.cm_mult.mult c0 (interp_vl r vm l0)) (interp_cs r vm s))
+let rec canonical_sum_scalar3_ok #a r vm c0 l0 s =
+  let aone  = r.cm_mult.unit in
+  let aplus = r.cm_add.mult in
+  let amult = r.cm_mult.mult in
+  match s with
+  | Cons_monom c l t ->
+    calc (==) {
+      interp_cs r vm (canonical_sum_scalar3 r c0 l0 s);
+      == { }
+      interp_cs r vm
+        (monom_insert r (amult c0 c) (varlist_merge l0 l)
+          (canonical_sum_scalar3 r c0 l0 t));
+      == { monom_insert_ok r vm (amult c0 c) (varlist_merge l0 l) (canonical_sum_scalar3 r c0 l0 t) }
+      aplus (amult (amult c0 c) (interp_vl r vm (varlist_merge l0 l)))
+            (interp_cs r vm (canonical_sum_scalar3 r c0 l0 t));
+      == { varlist_merge_ok r vm l0 l }
+      aplus (amult (amult c0 c) (amult (interp_vl r vm l0) (interp_vl r vm l)))
+            (interp_cs r vm (canonical_sum_scalar3 r c0 l0 t));
+      == { canonical_sum_scalar3_ok r vm c0 l0 t }
+      aplus (amult (amult c0 c) (amult (interp_vl r vm l0) (interp_vl r vm l)))
+            (amult (amult c0 (interp_vl r vm l0)) (interp_cs r vm t));
+      == { r.cm_mult.associativity (amult c0 c)
+             (interp_vl r vm l0) (interp_vl r vm l) }
+      aplus (amult (amult (amult c0 c) (interp_vl r vm l0)) (interp_vl r vm l))
+            (amult (amult c0 (interp_vl r vm l0)) (interp_cs r vm t));
+      == { r.cm_mult.commutativity c0 c }
+      aplus (amult (amult (amult c c0) (interp_vl r vm l0)) (interp_vl r vm l))
+            (amult (amult c0 (interp_vl r vm l0)) (interp_cs r vm t));
+      == { r.cm_mult.associativity c c0 (interp_vl r vm l0) }
+      aplus (amult (amult c (amult c0 (interp_vl r vm l0))) (interp_vl r vm l))
+            (amult (amult c0 (interp_vl r vm l0)) (interp_cs r vm t));
+      == { r.cm_mult.commutativity c (amult c0 (interp_vl r vm l0)) }
+      aplus (amult (amult (amult c0 (interp_vl r vm l0)) c) (interp_vl r vm l))
+            (amult (amult c0 (interp_vl r vm l0)) (interp_cs r vm t));
+      == { r.cm_mult.associativity (amult c0 (interp_vl r vm l0)) c (interp_vl r vm l) }
+      aplus (amult (amult c0 (interp_vl r vm l0)) (amult c (interp_vl r vm l)))
+            (amult (amult c0 (interp_vl r vm l0)) (interp_cs r vm t));
+      == { r.distribute (amult c0 (interp_vl r vm l0))
+             (amult c (interp_vl r vm l)) (interp_cs r vm t) }
+      amult (amult c0 (interp_vl r vm l0))
+            (aplus (amult c (interp_vl r vm l)) (interp_cs r vm t));
+      == {  }
+      amult (amult c0 (interp_vl r vm l0)) (interp_cs r vm s);
+    }
+  | Cons_varlist l t -> // Same as Cons_monom c l t with c = aone
+    let c = aone in
+    calc (==) {
+      interp_cs r vm (canonical_sum_scalar3 r c0 l0 s);
+      == { }
+      interp_cs r vm
+        (monom_insert r (amult c0 c) (varlist_merge l0 l)
+          (canonical_sum_scalar3 r c0 l0 t));
+      == { monom_insert_ok r vm (amult c0 c) (varlist_merge l0 l) (canonical_sum_scalar3 r c0 l0 t) }
+      aplus (amult (amult c0 c) (interp_vl r vm (varlist_merge l0 l)))
+            (interp_cs r vm (canonical_sum_scalar3 r c0 l0 t));
+      == { varlist_merge_ok r vm l0 l }
+      aplus (amult (amult c0 c) (amult (interp_vl r vm l0) (interp_vl r vm l)))
+            (interp_cs r vm (canonical_sum_scalar3 r c0 l0 t));
+      == { canonical_sum_scalar3_ok r vm c0 l0 t }
+      aplus (amult (amult c0 c) (amult (interp_vl r vm l0) (interp_vl r vm l)))
+            (amult (amult c0 (interp_vl r vm l0)) (interp_cs r vm t));
+      == { r.cm_mult.associativity (amult c0 c)
+             (interp_vl r vm l0) (interp_vl r vm l) }
+      aplus (amult (amult (amult c0 c) (interp_vl r vm l0)) (interp_vl r vm l))
+            (amult (amult c0 (interp_vl r vm l0)) (interp_cs r vm t));
+      == { r.cm_mult.commutativity c0 c }
+      aplus (amult (amult (amult c c0) (interp_vl r vm l0)) (interp_vl r vm l))
+            (amult (amult c0 (interp_vl r vm l0)) (interp_cs r vm t));
+      == { r.cm_mult.associativity c c0 (interp_vl r vm l0) }
+      aplus (amult (amult c (amult c0 (interp_vl r vm l0))) (interp_vl r vm l))
+            (amult (amult c0 (interp_vl r vm l0)) (interp_cs r vm t));
+      == { r.cm_mult.commutativity c (amult c0 (interp_vl r vm l0)) }
+      aplus (amult (amult (amult c0 (interp_vl r vm l0)) c) (interp_vl r vm l))
+            (amult (amult c0 (interp_vl r vm l0)) (interp_cs r vm t));
+      == { r.cm_mult.associativity (amult c0 (interp_vl r vm l0)) c (interp_vl r vm l) }
+      aplus (amult (amult c0 (interp_vl r vm l0)) (amult c (interp_vl r vm l)))
+            (amult (amult c0 (interp_vl r vm l0)) (interp_cs r vm t));
+      == { r.distribute (amult c0 (interp_vl r vm l0))
+             (amult c (interp_vl r vm l)) (interp_cs r vm t) }
+      amult (amult c0 (interp_vl r vm l0))
+            (aplus (amult c (interp_vl r vm l)) (interp_cs r vm t));
+      == {  }
+      amult (amult c0 (interp_vl r vm l0)) (interp_cs r vm s);
+    }
+  | Nil_monom -> ()
+
+val canonical_sum_prod_ok: #a:eqtype -> r:cr a -> vm:vmap a ->
+  s1:canonical_sum a -> s2:canonical_sum a ->
+  Lemma (interp_cs r vm (canonical_sum_prod r s1 s2) ==
+         r.cm_mult.mult (interp_cs r vm s1) (interp_cs r vm s2))
+let rec canonical_sum_prod_ok #a r vm s1 s2 =
+  let aone  = r.cm_mult.unit in
+  let aplus = r.cm_add.mult in
+  let amult = r.cm_mult.mult in
+  match s1 with
+  | Cons_monom c1 l1 t1 ->
+    calc (==) {
+      interp_cs r vm (canonical_sum_prod r s1 s2);
+      == { }
+      interp_cs r vm
+        (canonical_sum_merge r (canonical_sum_scalar3 r c1 l1 s2)
+                               (canonical_sum_prod r t1 s2));
+      == { canonical_sum_merge_ok r vm
+             (canonical_sum_scalar3 r c1 l1 s2)
+             (canonical_sum_prod r t1 s2) }
+      aplus (interp_cs r vm (canonical_sum_scalar3 r c1 l1 s2))
+            (interp_cs r vm (canonical_sum_prod r t1 s2));
+      == { canonical_sum_scalar3_ok r vm c1 l1 s2;
+           canonical_sum_prod_ok r vm t1 s2 }
+      aplus (amult (amult c1 (interp_vl r vm l1)) (interp_cs r vm s2))
+            (amult (interp_cs r vm t1) (interp_cs r vm s2));
+      == { distribute_right r (amult c1 (interp_vl r vm l1))
+             (interp_cs r vm t1) (interp_cs r vm s2) }
+      amult (aplus (amult c1 (interp_vl r vm l1)) (interp_cs r vm t1))
+            (interp_cs r vm s2);
+      == { }
+      amult (interp_cs r vm s1) (interp_cs r vm s2);
+    }
+  | Cons_varlist l1 t1 ->
+    calc (==) {
+      interp_cs r vm (canonical_sum_prod r s1 s2);
+      == { }
+      interp_cs r vm
+        (canonical_sum_merge r (canonical_sum_scalar2 r l1 s2)
+                               (canonical_sum_prod r t1 s2));
+      == { canonical_sum_merge_ok r vm
+             (canonical_sum_scalar2 r l1 s2)
+             (canonical_sum_prod r t1 s2) }
+      aplus (interp_cs r vm (canonical_sum_scalar2 r l1 s2))
+            (interp_cs r vm (canonical_sum_prod r t1 s2));
+      == { canonical_sum_scalar2_ok r vm l1 s2;
+           canonical_sum_prod_ok r vm t1 s2 }
+      aplus (amult (interp_vl r vm l1) (interp_cs r vm s2))
+            (amult (interp_cs r vm t1) (interp_cs r vm s2));
+      == { distribute_right r (interp_vl r vm l1)
+             (interp_cs r vm t1) (interp_cs r vm s2) }
+      amult (aplus (interp_vl r vm l1) (interp_cs r vm t1))
+            (interp_cs r vm s2);
+      == { }
+      amult (interp_cs r vm s1) (interp_cs r vm s2);
+    }
+  | Nil_monom -> ()
 
 val spolynomial_normalize_ok: #a:eqtype -> r:cr a -> vm:vmap a -> p:spolynomial a ->
   Lemma (interp_cs r vm (spolynomial_normalize r p) == interp_sp r vm p)
-let spolynomial_normalize_ok #a r vm p =
-  admit()
+let rec spolynomial_normalize_ok #a r vm p =
+  match p with
+  | SPvar _ -> ()
+  | SPconst _ -> ()
+  | SPplus l q ->
+    canonical_sum_merge_ok r vm
+      (spolynomial_normalize r l) (spolynomial_normalize r q);
+    spolynomial_normalize_ok r vm l;
+    spolynomial_normalize_ok r vm q
+  | SPmult l q ->
+    canonical_sum_prod_ok r vm
+      (spolynomial_normalize r l) (spolynomial_normalize r q);
+    spolynomial_normalize_ok r vm l;
+    spolynomial_normalize_ok r vm q
 
 val canonical_sum_simplify_ok: #a:eqtype -> r:cr a -> vm:vmap a -> s:canonical_sum a ->
   Lemma (interp_cs r vm (canonical_sum_simplify r s) == interp_cs r vm s)
-let canonical_sum_simplify_ok #a r vm s =
-  admit()
+let rec canonical_sum_simplify_ok #a r vm s =
+  let azero = r.cm_add.unit in
+  let aone  = r.cm_mult.unit in
+  match s with
+  | Cons_monom c _ t -> canonical_sum_simplify_ok r vm t
+  | Cons_varlist _ t -> canonical_sum_simplify_ok r vm t
+  | Nil_monom -> ()
 
 val spolynomial_simplify_ok: #a:eqtype -> r:cr a -> vm:vmap a -> p:spolynomial a ->
   Lemma (interp_cs r vm (spolynomial_simplify r p) == interp_sp r vm p)
@@ -605,23 +1310,42 @@ let spolynomial_simplify_ok #a r vm p =
   canonical_sum_simplify_ok r vm (spolynomial_normalize r p);
   spolynomial_normalize_ok r vm p
 
+///
+/// Tactic definition
+///
 
-/// Tactic
+(* Only dump when debugging is on *)
+let ddump m = if debugging () then dump m
 
-let make_fvar (#a:Type) (t:term) (unquotea:term -> Tac a) (ts:list term) (vm:vmap a) : Tac
-    (spolynomial a * list term * vmap a) =
-  match CCM.where t ts with
+(**
+ * Finds the position of first occurrence of x in xs.
+ * This is specialized to terms and their funny term_eq.
+**)
+let rec find_aux (n:nat) (x:term) (xs:list term) : Tot (option nat) (decreases xs) =
+  match xs with
+  | [] -> None
+  | x'::xs' -> if term_eq x x' then Some n else find_aux (n+1) x xs'
+
+let find = find_aux 0
+
+let make_fvar (#a:Type) (t:term) (unquotea:term -> Tac a) (ts:list term)
+  (vm:vmap a) : Tac (spolynomial a * list term * vmap a) =
+  match find t ts with
   | Some v -> (SPvar v, ts, vm)
   | None ->
     let vfresh = length ts in
     let z = unquotea t in
-    (SPvar vfresh, ts @ [t], CCM.update vfresh z () vm)
-
-// This expects that add, mult, and t have already been normalized
+    (SPvar vfresh, ts @ [t], update vfresh z vm)
+ 
+(** This expects that add, mult, and t have already been normalized *)
 let rec reification_aux (#a:Type) (unquotea:term -> Tac a) (ts:list term) (vm:vmap a) (add mult t: term) : Tac (spolynomial a * list term * vmap a) =
+  // dump ("term = " ^ term_to_string t ^ "\n");
   let hd, tl = collect_app_ref t in
   match inspect hd, list_unref tl with
-  | (Tv_FVar fv, [(t1, Q_Explicit) ; (t2, Q_Explicit)]) ->
+  | Tv_FVar fv, [(t1, _) ; (t2, _)] ->
+    //dump ("add = " ^ term_to_string add ^ "
+    //     \nmul = " ^ term_to_string mult);
+    //dump ("fv = " ^ term_to_string (pack (Tv_FVar fv)));
     let binop (op:spolynomial a -> spolynomial a -> spolynomial a) : Tac (spolynomial a * list term * vmap a) =
       let (e1, ts, vm) = reification_aux unquotea ts vm add mult t1 in
       let (e2, ts, vm) = reification_aux unquotea ts vm add mult t2 in
@@ -630,45 +1354,29 @@ let rec reification_aux (#a:Type) (unquotea:term -> Tac a) (ts:list term) (vm:vm
     if term_eq (pack (Tv_FVar fv)) add then binop SPplus else
     if term_eq (pack (Tv_FVar fv)) mult then binop SPmult else
     make_fvar t unquotea ts vm
-  | (_, _) -> make_fvar t unquotea ts vm
+  // Unquoting constants has issues when a <> int, 
+  // sometimes generates an unsolvable SMT goal
+  | Tv_Const _, [] -> SPconst (unquotea t), ts, vm
+  | _, _ -> make_fvar t unquotea ts vm
 
-let reification (#a:Type)
-    (unquotea:term->Tac a) (quotea:a -> Tac term) (tadd tmult:term) (munit:a) (ts:list term) :
-    Tac (list (spolynomial a) * vmap a) =
-  let add = norm_term [delta] tadd in
-  let mult = norm_term [delta] tmult in
-  let ts = Tactics.Util.map (norm_term [delta]) ts in
-  //ddump ("add = " ^ term_to_string add ^ "; mult = " ^ term_to_string mult);
-  let (es, _, vm) =
-    Tactics.Util.fold_left
-      (fun (es,vs,vm) t ->
-        let (e,vs,vm) = reification_aux unquotea vs vm add mult t
-        in (e::es,vs,vm))
-      ([],[], ([], (munit, ()))) ts
-  in (List.rev es,vm)
-
-let canon_norm () : Tac unit =
-  norm [
+(** 
+ * How to normalize terms in the tactic.
+ * This is carefully tuned to unfold all and no more than required
+**)
+let steps =
+  [
     primops;
     iota;
     zeta;
     delta_attr [`%canon_attr];
     delta_only [
-      "FStar.Algebra.CommMonoid.int_plus_cm";
-      "FStar.Algebra.CommMonoid.int_multiply_cm";
+      "FStar.Mul.op_Star";                        // For integer ring
+      "FStar.Algebra.CommMonoid.int_plus_cm";     // For integer ring
+      "FStar.Algebra.CommMonoid.int_multiply_cm"; // For integer ring
       "FStar.Algebra.CommMonoid.__proj__CM__item__mult";
       "FStar.Algebra.CommMonoid.__proj__CM__item__unit";
       "FStar.Tactics.CanonCommSemiring.__proj__CR__item__cm_add";
       "FStar.Tactics.CanonCommSemiring.__proj__CR__item__cm_mult";
-      "FStar.Tactics.CanonCommMonoid.canon";
-      "FStar.Tactics.CanonCommMonoid.xsdenote";
-      "FStar.Tactics.CanonCommMonoid.flatten";
-      "FStar.Tactics.CanonCommMonoid.select";
-      "FStar.Tactics.CanonCommMonoid.select_extra";
-      "FStar.Tactics.CanonCommMonoid.const_last";
-      "FStar.Tactics.CanonCommMonoid.const_compare";
-      "FStar.Tactics.CanonCommMonoid.special_compare";
-      "FStar.Tactics.CanonCommMonoid.sortWith_correct";
       "FStar.List.Tot.Base.assoc";
       "FStar.Pervasives.Native.fst";
       "FStar.Pervasives.Native.snd";
@@ -676,13 +1384,27 @@ let canon_norm () : Tac unit =
       "FStar.Pervasives.Native.__proj__Mktuple2__item___2";
       "FStar.List.Tot.Base.op_At";
       "FStar.List.Tot.Base.append";
-      "FStar.List.Tot.Base.sortWith";
-      "FStar.List.Tot.Base.partition";
-      "FStar.List.Tot.Base.bool_of_compare";
-      "FStar.List.Tot.Base.compare_of_bool";
     ]
   ]
 
+let canon_norm () : Tac unit = norm steps
+
+let reification (#a:Type)
+  (unquotea:term -> Tac a) (quotea:a -> Tac term) (tadd tmult:term) (munit:a) (ts:list term) : Tac (list (spolynomial a) * vmap a) =
+  // Be careful not to normalize operations too much
+  // E.g. we don't want to turn ( +% ) into (a + b ) % prime
+  // or we won't be able to spot ring operations
+  let add  = tadd in
+  let mult = tmult in
+  let ts = Tactics.Util.map (norm_term steps) ts in
+  //ddump ("add = " ^ term_to_string add ^ "\nmult = " ^ term_to_string mult);
+  let (es, _, vm) =
+    Tactics.Util.fold_left
+      (fun (es, vs, vm) t ->
+        let (e, vs, vm) = reification_aux unquotea vs vm add mult t
+        in (e::es, vs, vm))
+      ([],[], ([], munit)) ts
+  in (List.rev es, vm)
 
 let rec quote_spolynomial (#a:Type) (e:spolynomial a) : Tac term =
   match e with
@@ -691,12 +1413,13 @@ let rec quote_spolynomial (#a:Type) (e:spolynomial a) : Tac term =
   | SPplus e1 e2 -> mk_e_app (`SPplus) [quote_spolynomial e1; quote_spolynomial e2]
   | SPmult e1 e2 -> mk_e_app (`SPmult) [quote_spolynomial e1; quote_spolynomial e2]
 
+(* Constructs the 3 main goals of the tactic *)
 let semiring_reflect (#a:eqtype) (r:cr a) (vm:vmap a) (e1 e2:spolynomial a) (a1 a2:a)
     (_ : squash (
-      interp_cs r vm (spolynomial_simplify r e1) ==
-      interp_cs r vm (spolynomial_simplify r e2)))
-    (_ : squash (a1 == interp_sp r vm e1))
-    (_ : squash (a2 == interp_sp r vm e2)) :
+      interp_cs r vm (spolynomial_simplify #a r e1) ==
+      interp_cs r vm (spolynomial_simplify #a r e2)))
+    (_ : squash (a1 == interp_sp #a r vm e1))
+    (_ : squash (a2 == interp_sp #a r vm e2)) :
     squash (a1 == a2)
   =
   spolynomial_simplify_ok r vm e1;
@@ -705,114 +1428,169 @@ let semiring_reflect (#a:eqtype) (r:cr a) (vm:vmap a) (e1 e2:spolynomial a) (a1 
 [@plugin]
 let canon_semiring_aux
     (a: Type) (ta: term) (unquotea: term -> Tac a) (quotea: a -> Tac term)
-    (tr tadd tmult: term) (munit: a) (tb: term)
-  : Tac unit =
+    (tr tadd tmult: term) (munit: a)
+  : Tac unit
+=
   focus (fun () ->
-  norm [];
+  norm []; // Do not normalize anything implicitly
   let g = cur_goal () in
   match term_as_formula g with
   | Comp (Eq (Some t)) t1 t2 ->
-    (
-      //ddump ("t1 = " ^ term_to_string t1 ^ "; t2 = " ^ term_to_string t2);
+    begin
+      //ddump ("t1 = " ^ term_to_string t1 ^ "\nt2 = " ^ term_to_string t2);
       if term_eq t ta then
-      (
-        match reification unquotea quotea tadd tmult munit [t1; t2] with
-        | ([e1; e2], vm) ->
-          (
-(*
-            let r : cr a = unquote tr in
-            ddump (
-              "e1 = " ^ exp_to_string e1 ^
-              "; e2 = " ^ exp_to_string e2);
-            ddump ("vm = " ^ term_to_string (quote vm));
-            ddump ("before = " ^ term_to_string (norm_term [delta; primops]
-              (quote (rdenote r vm e1 == rdenote r vm e2))));
-            ddump ("expected after = " ^ term_to_string (norm_term [delta; primops]
-              (quote (
-                cdenote p r vm (exp_to_sum e1) ==
-                cdenote p r vm (exp_to_sum e2)))));
-*)
-            // let q_app0 = quote (semiring_reflect #a #b p pc r vm e1 e2) in
-            ddump (term_to_string t1);
-            let tvm = CCM.quote_vm ta tb quotea (fun _ -> `()) vm in
-            let te1 = quote_spolynomial e1 in
-            // ddump (exp_to_string e1);
-            // ddump (term_to_string te1);
-            let te2 = quote_spolynomial e2 in
-            // ddump (term_to_string te2);
-            mapply (`(semiring_reflect #(`#ta) (`#tr) (`#tvm) (`#te1) (`#te2) (`#t1) (`#t2)));
-            //unfold_def tp;
-            canon_norm ();
-            later ();
-            canon_norm ();
-            ddump ("after norm-left");
-            trefl ();
-            canon_norm ();
-            ddump ("after norm-right");
-            trefl ();
-            (* ddump "done"; *)
-            ()
-          )
-        | _ -> fail "Unexpected"
-      )
+      begin
+      match reification unquotea quotea tadd tmult munit [t1; t2] with
+      | ([e1; e2], vm) ->
+        //ddump (term_to_string t1);
+        //ddump (term_to_string t2);
+        //
+        //let r : cr a = unquote tr in
+        //ddump ("e1 = " ^ exp_to_string e1 ^ "\ne2 = " ^ exp_to_string e2);
+        dump ("vm = " ^ term_to_string (quote vm));
+        //ddump ("before = " ^ term_to_string (norm_term [delta; primops]
+        //  (quote (interp_sp r vm e1 == interp_sp r vm e2))));
+        //ddump ("expected after = " ^ term_to_string (norm_term [delta; primops]
+        //  (quote (
+        //    interp_vs r vm (spolynomial_simplify r e1) ==
+        //    interp_vs r vm (spolynomial_simplify r e2))));
+        let tvm = quote_vm ta quotea vm in
+        let te1 = quote_spolynomial e1 in
+        //dump ("te1 = " ^ term_to_string te1);
+        let te2 = quote_spolynomial e2 in
+        //dump ("te2 = " ^ term_to_string te2);
+        mapply (`(semiring_reflect
+          #(`#ta) (`#tr) (`#tvm) (`#te1) (`#te2) (`#t1) (`#t2)));
+        //dump "Before norm1";
+        canon_norm ();
+        //dump "After norm1";
+        later ();
+        //dump "Before norm2";
+        canon_norm ();
+        //dump "After norm2";
+        //ddump ("after normalizing left-hand side");
+        trefl ();
+        //dump "Before norm3";
+        canon_norm ();
+        //dump "After norm3";
+        //ddump ("after normalizing right-hand side");
+        trefl ()
+      | _ -> fail "Unexpected"
+      end
       else fail "Found equality, but terms do not have the expected type"
-    )
+    end
   | _ -> fail "Goal should be an equality")
 
 
-let canon_semiring_with (#a:Type) (r:cr a) : Tac unit =
+let canon_semiring (#a:eqtype) (r:cr a) : Tac unit =
   canon_semiring_aux a
-    (quote a) (unquote #a) (fun (x:a) -> quote x)
-    (quote r) (quote (cm_op (r.cm_add))) (quote (cm_op (r.cm_mult))) (CM?.unit (r.cm_add)) (quote unit)
+    (quote a) (unquote #a) (fun (x:a) -> quote x) (quote r) 
+    (quote r.cm_add.mult) (quote r.cm_mult.mult) r.cm_add.unit
 
-let canon_semiring (#a:Type) (r:cr a) : Tac unit =
-  canon_semiring_with r
+let canon_semiring_with (#a:eqtype) (r:cr a) (add:a -> a -> a) (mul:a -> a -> a) 
+  : Tac unit =
+  canon_semiring_aux a
+    (quote a) (unquote #a) (fun (x:a) -> quote x) (quote r) 
+    (quote add) (quote mul) r.cm_add.unit
 
-
+///
 /// Examples
+///
 
 open FStar.Mul
 
-#set-options "--no_smt"
+///  Ring of integers
 
-let poly (a b c:int) =
-  assert ( a * b + c + b * b == (b + a) * b + c)
-  by (canon_semiring int_cr)
+[@canon_attr]
+let int_cr : cr int =
+  CR int_plus_cm int_multiply_cm (fun x y z -> ()) (fun x -> ())
 
-assume
-val ring: eqtype
+#push-options "--no_smt --tactic_trace_d 1" // Look, no SMT!
 
-assume
-val zero: ring
+let semiring () : Tac unit =
+  canon_semiring_with #int int_cr Prims.op_Addition Prims.op_Multiply
 
-assume
-val one: ring
+let test1 (a:int) =
+  assert (a + a == 2 * a) by (semiring ())
 
-assume
-val ( +. ) : a:ring -> b:ring -> ring
+let test2 (a b:int) =
+  assert (b + a + a + a + 4 + a + 3 * (a + b) + 7 == 
+          a * 3 + 2 * b + b + a + b * 1 + 7 + (2 + 1) * a + 4) 
+  by (semiring ()) 
 
-assume
-val ( *. ) : a:ring -> b:ring -> ring
+let test3 (a b c:int) =
+  assert (a * b + c + b * b == (b + a) * b + c) by (semiring()) 
 
-assume
+#pop-options
+
+/// Ring of integers modulo 2^130 - 5 (the Poly1305 prime)
+
+#set-options "--z3rlimit 10 --max_fuel 0 --max_ifuel 0"
+
+let prime: pos =
+  normalize_term_spec (pow2 130 - 5);
+  pow2 130 - 5
+
+let ring : eqtype = a:nat{a < prime}
+
+[@canon_attr]
+let zero : ring = 0
+
+[@canon_attr]
+let one : ring = normalize_term_spec prime; 1
+
+//[@(strict_on_arguments [0;1])]
+let ( +. ) (a b:ring) : ring = (a + b) % prime
+
+//[@(strict_on_arguments [0;1])]
+let ( *. ) (a b:ring) : ring = (a * b) % prime
+
 val add_identity: a:ring -> Lemma (zero +. a == a)
+let add_identity a = normalize_term_spec prime
 
-assume
+val mul_identity: a:ring -> Lemma (one *. a == a)
+let mul_identity a = normalize_term_spec prime
+
+#set-options "--z3cliopt smt.arith.nl=false"
+
 val add_associativity: a:ring -> b:ring -> c:ring
   -> Lemma (a +. b +. c == a +. (b +. c))
+let add_associativity a b c =
+  normalize_term_spec prime;
+  calc (==) {
+    a +. b +. c;
+    == { }
+    ((a + b) % prime + c) % prime;
+    == { Math.Lemmas.lemma_mod_plus_distr_l (a + b) c prime }
+    ((a + b) + c) % prime;
+    == { }
+    (a + (b + c)) % prime;
+    == { Math.Lemmas.lemma_mod_plus_distr_r a (b + c) prime }
+    a +. (b +. c);
+  }
 
-assume
 val add_commutativity: a:ring -> b:ring -> Lemma (a +. b == b +. a)
+let add_commutativity a b = ()
 
-assume
-val mul_identity: a:ring -> Lemma (one *. a == a)
-
-assume
 val mul_associativity: a:ring -> b:ring -> c:ring
   -> Lemma (a *. b *. c == a *. (b *. c))
+let mul_associativity a b c =
+  calc (==) {
+    a *. b *. c;
+    == { }
+    (((a * b) % prime) * c) % prime;
+    == { Math.Lemmas.lemma_mod_mul_distr_l (a * b) c prime }
+    ((a * b) * c) % prime;
+    == { Math.Lemmas.paren_mul_right a b c }
+    (a * (b * c)) % prime;
+    == { Math.Lemmas.lemma_mod_mul_distr_r a (b * c) prime }
+    (a * ((b * c) % prime)) % prime;
+    == { }
+    a *. (b *. c);
+  }
 
-assume
 val mul_commutativity: a:ring -> b:ring -> Lemma (a *. b == b *. a)
+let mul_commutativity a b = ()
 
 [@canon_attr]
 let ring_add_cm : cm ring =
@@ -822,19 +1600,52 @@ let ring_add_cm : cm ring =
 let ring_mul_cm : cm ring =
   CM one ( *. ) mul_identity mul_associativity mul_commutativity
 
-assume
 val mul_add_distr: distribute_left_lemma ring ring_add_cm ring_mul_cm
+let mul_add_distr a b c =
+  normalize_term_spec prime;
+  calc (==) {
+    a *. (b +. c);
+    == { }
+    (a * (b +. c)) % prime;
+    == { Math.Lemmas.lemma_mod_add_distr a (b + c) prime }
+    (a * ((b + c) % prime)) % prime;
+    == { Math.Lemmas.lemma_mod_mul_distr_r a (b + c) prime }
+    (a * (b + c)) % prime;
+    == { Math.Lemmas.distributivity_add_right a b c }
+    (a * b + a * c) % prime;
+    == { Math.Lemmas.lemma_mod_add_distr (a * b) (a * c) prime }
+    (a * b + a *. c) % prime;
+    == { }
+    (a *. c + a * b) % prime;
+    == { Math.Lemmas.lemma_mod_add_distr (a *. c) (a * b) prime }
+    (a *. c + a *. b) % prime;
+    == { }
+    (a *. b + a *. c) % prime;
+    == { }
+    a *. b +. a *. c;
+  }
+
+val mul_zero_l: mult_zero_l_lemma ring ring_add_cm ring_mul_cm
+let mul_zero_l a = assert_norm (0 % prime == 0)
 
 [@canon_attr]
-let ring_cr : cr ring = CR ring_add_cm ring_mul_cm mul_add_distr
+let ring_cr : cr ring = CR ring_add_cm ring_mul_cm mul_add_distr mul_zero_l
 
-#reset-options "--max_fuel 0 --max_ifuel 0 --z3rlimit 1"
+let semiring_poly () : Tac unit = canon_semiring_with ring_cr ( +. ) ( *. )
 
-let poly_update_repeat_blocks_multi_lemma2_simplify (a b c w r d:ring) : Lemma
-  ((((a *. (r *. r)) +. c) *. (r *. r)) +. ((b *. (r *. r)) +. d) *. r ==
-   (((((a *. (r *. r)) +. b *. r) +. c) *. r) +. d) *. r)
+let poly (a b:ring) =
+  assert (a +. b == b +. a) by (semiring_poly ())
+
+#set-options "--tactic_trace_d 1"
+
+[@tcdecltime]
+let poly_update_repeat_blocks_multi_lemma2_simplify (a b c w r d:ring) :
+  Lemma
+  ( (((a *. (r *. r)) +. c) *. (r *. r)) +. ((b *. (r *. r)) +. d) *. r ==
+    (((((a *. (r *. r)) +. b *. r) +. c) *. r) +. d) *. r)
 =
+  normalize_term_spec prime;
   assert (
     (((a *. (r *. r)) +. c) *. (r *. r)) +. ((b *. (r *. r)) +. d) *. r ==
     ((a *. (r *. r) +. b *. r +. c) *. r +. d) *. r)
-  by (canon_semiring ring_cr)
+  by (semiring_poly ())
